Mathbin/Data/Rbtree/Insert.lean
@@ -12,106 +12,120 @@ import Mathbin.Data.Rbtree.Find
 
 universe u v
 
-attribute [local simp] Rbnode.Lift
+attribute [local simp] Std.RBNode.Lift
 
-namespace Rbnode
+namespace Std.RBNode
 
 variable {α : Type u}
 
 open Color
 
 @[simp]
-theorem balance1_eq₁ (l : Rbnode α) (x r₁ y r₂ v t) :
-    balance1 (red_node l x r₁) y r₂ v t = red_node (black_node l x r₁) y (black_node r₂ v t) := by
-  cases r₂ <;> rfl
-#align rbnode.balance1_eq₁ Rbnode.balance1_eq₁
+theorem Std.RBNode.balance1_eq₁ (l : Std.RBNode α) (x r₁ y r₂ v t) :
+    Std.RBNode.balance1 (Std.RBNode.node l x r₁) y r₂ v t =
+      Std.RBNode.node (black_node l x r₁) y (black_node r₂ v t) :=
+  by cases r₂ <;> rfl
+#align rbnode.balance1_eq₁ Std.RBNode.balance1_eq₁
 
 @[simp]
-theorem balance1_eq₂ (l₁ : Rbnode α) (y l₂ x r v t) :
-    getColor l₁ ≠ red →
-      balance1 l₁ y (red_node l₂ x r) v t = red_node (black_node l₁ y l₂) x (black_node r v t) :=
+theorem Std.RBNode.balance1_eq₂ (l₁ : Std.RBNode α) (y l₂ x r v t) :
+    Std.RBNode.getColor l₁ ≠ red →
+      Std.RBNode.balance1 l₁ y (Std.RBNode.node l₂ x r) v t =
+        Std.RBNode.node (black_node l₁ y l₂) x (black_node r v t) :=
   by cases l₁ <;> simp [get_color, balance1, false_imp_iff]
-#align rbnode.balance1_eq₂ Rbnode.balance1_eq₂
+#align rbnode.balance1_eq₂ Std.RBNode.balance1_eq₂
 
 @[simp]
-theorem balance1_eq₃ (l : Rbnode α) (y r v t) :
-    getColor l ≠ red → getColor r ≠ red → balance1 l y r v t = black_node (red_node l y r) v t := by
-  cases l <;> cases r <;> simp [get_color, balance1, false_imp_iff]
-#align rbnode.balance1_eq₃ Rbnode.balance1_eq₃
+theorem Std.RBNode.balance1_eq₃ (l : Std.RBNode α) (y r v t) :
+    Std.RBNode.getColor l ≠ red →
+      Std.RBNode.getColor r ≠ red →
+        Std.RBNode.balance1 l y r v t = black_node (Std.RBNode.node l y r) v t :=
+  by cases l <;> cases r <;> simp [get_color, balance1, false_imp_iff]
+#align rbnode.balance1_eq₃ Std.RBNode.balance1_eq₃
 
 @[simp]
-theorem balance2_eq₁ (l : Rbnode α) (x₁ r₁ y r₂ v t) :
-    balance2 (red_node l x₁ r₁) y r₂ v t = red_node (black_node t v l) x₁ (black_node r₁ y r₂) := by
-  cases r₂ <;> rfl
-#align rbnode.balance2_eq₁ Rbnode.balance2_eq₁
+theorem Std.RBNode.balance2_eq₁ (l : Std.RBNode α) (x₁ r₁ y r₂ v t) :
+    Std.RBNode.balance2 (Std.RBNode.node l x₁ r₁) y r₂ v t =
+      Std.RBNode.node (black_node t v l) x₁ (black_node r₁ y r₂) :=
+  by cases r₂ <;> rfl
+#align rbnode.balance2_eq₁ Std.RBNode.balance2_eq₁
 
 @[simp]
-theorem balance2_eq₂ (l₁ : Rbnode α) (y l₂ x₂ r₂ v t) :
-    getColor l₁ ≠ red →
-      balance2 l₁ y (red_node l₂ x₂ r₂) v t =
-        red_node (black_node t v l₁) y (black_node l₂ x₂ r₂) :=
+theorem Std.RBNode.balance2_eq₂ (l₁ : Std.RBNode α) (y l₂ x₂ r₂ v t) :
+    Std.RBNode.getColor l₁ ≠ red →
+      Std.RBNode.balance2 l₁ y (Std.RBNode.node l₂ x₂ r₂) v t =
+        Std.RBNode.node (black_node t v l₁) y (black_node l₂ x₂ r₂) :=
   by cases l₁ <;> simp [get_color, balance2, false_imp_iff]
-#align rbnode.balance2_eq₂ Rbnode.balance2_eq₂
+#align rbnode.balance2_eq₂ Std.RBNode.balance2_eq₂
 
 @[simp]
-theorem balance2_eq₃ (l : Rbnode α) (y r v t) :
-    getColor l ≠ red → getColor r ≠ red → balance2 l y r v t = black_node t v (red_node l y r) := by
-  cases l <;> cases r <;> simp [get_color, balance2, false_imp_iff]
-#align rbnode.balance2_eq₃ Rbnode.balance2_eq₃
+theorem Std.RBNode.balance2_eq₃ (l : Std.RBNode α) (y r v t) :
+    Std.RBNode.getColor l ≠ red →
+      Std.RBNode.getColor r ≠ red →
+        Std.RBNode.balance2 l y r v t = black_node t v (Std.RBNode.node l y r) :=
+  by cases l <;> cases r <;> simp [get_color, balance2, false_imp_iff]
+#align rbnode.balance2_eq₃ Std.RBNode.balance2_eq₃
 
 -- We can use the same induction principle for balance1 and balance2
-theorem Balance.cases {p : Rbnode α → α → Rbnode α → Prop} (l y r)
-    (red_left : ∀ l x r₁ y r₂, p (red_node l x r₁) y r₂)
-    (red_right : ∀ l₁ y l₂ x r, getColor l₁ ≠ red → p l₁ y (red_node l₂ x r))
-    (other : ∀ l y r, getColor l ≠ red → getColor r ≠ red → p l y r) : p l y r :=
-  by
+theorem Std.RBNode.Balance.cases {p : Std.RBNode α → α → Std.RBNode α → Prop} (l y r)
+    (red_left : ∀ l x r₁ y r₂, p (Std.RBNode.node l x r₁) y r₂)
+    (red_right : ∀ l₁ y l₂ x r, Std.RBNode.getColor l₁ ≠ red → p l₁ y (Std.RBNode.node l₂ x r))
+    (other : ∀ l y r, Std.RBNode.getColor l ≠ red → Std.RBNode.getColor r ≠ red → p l y r) :
+    p l y r := by
   cases l <;> cases r
   any_goals apply red_left
   any_goals apply red_right <;> simp [get_color] <;> contradiction <;> done
   any_goals apply other <;> simp [get_color] <;> contradiction <;> done
-#align rbnode.balance.cases Rbnode.Balance.cases
+#align rbnode.balance.cases Std.RBNode.Balance.cases
 
-theorem balance1_ne_leaf (l : Rbnode α) (x r v t) : balance1 l x r v t ≠ leaf := by
+theorem Std.RBNode.balance1_ne_nil (l : Std.RBNode α) (x r v t) :
+    Std.RBNode.balance1 l x r v t ≠ Std.RBNode.nil := by
   apply balance.cases l x r <;> intros <;> simp [*] <;> contradiction
-#align rbnode.balance1_ne_leaf Rbnode.balance1_ne_leaf
+#align rbnode.balance1_ne_leaf Std.RBNode.balance1_ne_nil
 
-theorem balance1Node_ne_leaf {s : Rbnode α} (a : α) (t : Rbnode α) :
-    s ≠ leaf → balance1Node s a t ≠ leaf := by
+theorem Std.RBNode.balance1Node_ne_nil {s : Std.RBNode α} (a : α) (t : Std.RBNode α) :
+    s ≠ Std.RBNode.nil → Std.RBNode.balance1Node s a t ≠ Std.RBNode.nil :=
+  by
   intro h; cases s
   · contradiction
   all_goals simp [balance1_node]; apply balance1_ne_leaf
-#align rbnode.balance1_node_ne_leaf Rbnode.balance1Node_ne_leaf
+#align rbnode.balance1_node_ne_leaf Std.RBNode.balance1Node_ne_nil
 
-theorem balance2_ne_leaf (l : Rbnode α) (x r v t) : balance2 l x r v t ≠ leaf := by
+theorem Std.RBNode.balance2_ne_nil (l : Std.RBNode α) (x r v t) :
+    Std.RBNode.balance2 l x r v t ≠ Std.RBNode.nil := by
   apply balance.cases l x r <;> intros <;> simp [*] <;> contradiction
-#align rbnode.balance2_ne_leaf Rbnode.balance2_ne_leaf
+#align rbnode.balance2_ne_leaf Std.RBNode.balance2_ne_nil
 
-theorem balance2Node_ne_leaf {s : Rbnode α} (a : α) (t : Rbnode α) :
-    s ≠ leaf → balance2Node s a t ≠ leaf := by
+theorem Std.RBNode.balance2Node_ne_nil {s : Std.RBNode α} (a : α) (t : Std.RBNode α) :
+    s ≠ Std.RBNode.nil → Std.RBNode.balance2Node s a t ≠ Std.RBNode.nil :=
+  by
   intro h; cases s
   · contradiction
   all_goals simp [balance2_node]; apply balance2_ne_leaf
-#align rbnode.balance2_node_ne_leaf Rbnode.balance2Node_ne_leaf
+#align rbnode.balance2_node_ne_leaf Std.RBNode.balance2Node_ne_nil
 
 variable (lt : α → α → Prop)
 
 @[elab_as_elim]
-theorem ins.induction [DecidableRel lt] {p : Rbnode α → Prop} (t x) (is_leaf : p leaf)
-    (is_red_lt : ∀ (a y b) (hc : cmpUsing lt x y = Ordering.lt) (ih : p a), p (red_node a y b))
-    (is_red_eq : ∀ (a y b) (hc : cmpUsing lt x y = Ordering.eq), p (red_node a y b))
-    (is_red_gt : ∀ (a y b) (hc : cmpUsing lt x y = Ordering.gt) (ih : p b), p (red_node a y b))
+theorem Std.RBNode.ins.induction [DecidableRel lt] {p : Std.RBNode α → Prop} (t x)
+    (is_leaf : p Std.RBNode.nil)
+    (is_red_lt :
+      ∀ (a y b) (hc : cmpUsing lt x y = Ordering.lt) (ih : p a), p (Std.RBNode.node a y b))
+    (is_red_eq : ∀ (a y b) (hc : cmpUsing lt x y = Ordering.eq), p (Std.RBNode.node a y b))
+    (is_red_gt :
+      ∀ (a y b) (hc : cmpUsing lt x y = Ordering.gt) (ih : p b), p (Std.RBNode.node a y b))
     (is_black_lt_red :
-      ∀ (a y b) (hc : cmpUsing lt x y = Ordering.lt) (hr : getColor a = red) (ih : p a),
+      ∀ (a y b) (hc : cmpUsing lt x y = Ordering.lt) (hr : Std.RBNode.getColor a = red) (ih : p a),
         p (black_node a y b))
     (is_black_lt_not_red :
-      ∀ (a y b) (hc : cmpUsing lt x y = Ordering.lt) (hnr : getColor a ≠ red) (ih : p a),
+      ∀ (a y b) (hc : cmpUsing lt x y = Ordering.lt) (hnr : Std.RBNode.getColor a ≠ red) (ih : p a),
         p (black_node a y b))
     (is_black_eq : ∀ (a y b) (hc : cmpUsing lt x y = Ordering.eq), p (black_node a y b))
     (is_black_gt_red :
-      ∀ (a y b) (hc : cmpUsing lt x y = Ordering.gt) (hr : getColor b = red) (ih : p b),
+      ∀ (a y b) (hc : cmpUsing lt x y = Ordering.gt) (hr : Std.RBNode.getColor b = red) (ih : p b),
         p (black_node a y b))
     (is_black_gt_not_red :
-      ∀ (a y b) (hc : cmpUsing lt x y = Ordering.gt) (hnr : getColor b ≠ red) (ih : p b),
+      ∀ (a y b) (hc : cmpUsing lt x y = Ordering.gt) (hnr : Std.RBNode.getColor b ≠ red) (ih : p b),
         p (black_node a y b)) :
     p t := by
   induction t
@@ -132,24 +146,26 @@ theorem ins.induction [DecidableRel lt] {p : Rbnode α → Prop} (t x) (is_leaf 
       by_cases get_color b = red
       · apply is_black_gt_red <;> assumption
       · apply is_black_gt_not_red <;> assumption
-#align rbnode.ins.induction Rbnode.ins.induction
+#align rbnode.ins.induction Std.RBNode.ins.induction
 
 /- ./././Mathport/Syntax/Translate/Tactic/Builtin.lean:69:18: unsupported non-interactive tactic rbnode.is_searchable_tactic -/
-theorem isSearchable_balance1 {l y r v t lo hi} :
-    IsSearchable lt l lo (some y) →
-      IsSearchable lt r (some y) (some v) →
-        IsSearchable lt t (some v) hi → IsSearchable lt (balance1 l y r v t) lo hi :=
+theorem Std.RBNode.isSearchableBalance1 {l y r v t lo hi} :
+    Std.RBNode.IsSearchable lt l lo (some y) →
+      Std.RBNode.IsSearchable lt r (some y) (some v) →
+        Std.RBNode.IsSearchable lt t (some v) hi →
+          Std.RBNode.IsSearchable lt (Std.RBNode.balance1 l y r v t) lo hi :=
   by
   apply balance.cases l y r <;> intros <;> simp [*] <;>
     run_tac
       is_searchable_tactic
-#align rbnode.is_searchable_balance1 Rbnode.isSearchable_balance1
+#align rbnode.is_searchable_balance1 Std.RBNode.isSearchableBalance1
 
 /- ./././Mathport/Syntax/Translate/Tactic/Builtin.lean:69:18: unsupported non-interactive tactic rbnode.is_searchable_tactic -/
-theorem isSearchable_balance1Node {t} [IsTrans α lt] :
+theorem Std.RBNode.isSearchableBalance1Node {t} [IsTrans α lt] :
     ∀ {y s lo hi},
-      IsSearchable lt t lo (some y) →
-        IsSearchable lt s (some y) hi → IsSearchable lt (balance1Node t y s) lo hi :=
+      Std.RBNode.IsSearchable lt t lo (some y) →
+        Std.RBNode.IsSearchable lt s (some y) hi →
+          Std.RBNode.IsSearchable lt (Std.RBNode.balance1Node t y s) lo hi :=
   by
   cases t <;> simp! <;> intros <;>
     run_tac
@@ -158,24 +174,26 @@ theorem isSearchable_balance1Node {t} [IsTrans α lt] :
     · apply is_searchable_none_low_of_is_searchable_some_low; assumption
     · simp at *; apply is_searchable_some_low_of_is_searchable_of_lt <;> assumption
   all_goals apply is_searchable_balance1 <;> assumption
-#align rbnode.is_searchable_balance1_node Rbnode.isSearchable_balance1Node
+#align rbnode.is_searchable_balance1_node Std.RBNode.isSearchableBalance1Node
 
 /- ./././Mathport/Syntax/Translate/Tactic/Builtin.lean:69:18: unsupported non-interactive tactic rbnode.is_searchable_tactic -/
-theorem isSearchable_balance2 {l y r v t lo hi} :
-    IsSearchable lt t lo (some v) →
-      IsSearchable lt l (some v) (some y) →
-        IsSearchable lt r (some y) hi → IsSearchable lt (balance2 l y r v t) lo hi :=
+theorem Std.RBNode.isSearchableBalance2 {l y r v t lo hi} :
+    Std.RBNode.IsSearchable lt t lo (some v) →
+      Std.RBNode.IsSearchable lt l (some v) (some y) →
+        Std.RBNode.IsSearchable lt r (some y) hi →
+          Std.RBNode.IsSearchable lt (Std.RBNode.balance2 l y r v t) lo hi :=
   by
   apply balance.cases l y r <;> intros <;> simp [*] <;>
     run_tac
       is_searchable_tactic
-#align rbnode.is_searchable_balance2 Rbnode.isSearchable_balance2
+#align rbnode.is_searchable_balance2 Std.RBNode.isSearchableBalance2
 
 /- ./././Mathport/Syntax/Translate/Tactic/Builtin.lean:69:18: unsupported non-interactive tactic rbnode.is_searchable_tactic -/
-theorem isSearchable_balance2Node {t} [IsTrans α lt] :
+theorem Std.RBNode.isSearchableBalance2Node {t} [IsTrans α lt] :
     ∀ {y s lo hi},
-      IsSearchable lt s lo (some y) →
-        IsSearchable lt t (some y) hi → IsSearchable lt (balance2Node t y s) lo hi :=
+      Std.RBNode.IsSearchable lt s lo (some y) →
+        Std.RBNode.IsSearchable lt t (some y) hi →
+          Std.RBNode.IsSearchable lt (Std.RBNode.balance2Node t y s) lo hi :=
   by
   induction t <;> simp! <;> intros <;>
     run_tac
@@ -184,12 +202,13 @@ theorem isSearchable_balance2Node {t} [IsTrans α lt] :
     · apply is_searchable_none_high_of_is_searchable_some_high; assumption
     · simp at *; apply is_searchable_some_high_of_is_searchable_of_lt; assumption'
   all_goals apply is_searchable_balance2; assumption'
-#align rbnode.is_searchable_balance2_node Rbnode.isSearchable_balance2Node
+#align rbnode.is_searchable_balance2_node Std.RBNode.isSearchableBalance2Node
 
 /- ./././Mathport/Syntax/Translate/Tactic/Builtin.lean:69:18: unsupported non-interactive tactic rbnode.is_searchable_tactic -/
-theorem isSearchable_ins [DecidableRel lt] {t x} [IsStrictWeakOrder α lt] :
-    ∀ {lo hi} (h : IsSearchable lt t lo hi),
-      Lift lt lo (some x) → Lift lt (some x) hi → IsSearchable lt (ins lt t x) lo hi :=
+theorem Std.RBNode.isSearchableIns [DecidableRel lt] {t x} [IsStrictWeakOrder α lt] :
+    ∀ {lo hi} (h : Std.RBNode.IsSearchable lt t lo hi),
+      Std.RBNode.Lift lt lo (some x) →
+        Std.RBNode.Lift lt (some x) hi → Std.RBNode.IsSearchable lt (Std.RBNode.ins lt t x) lo hi :=
   by
   apply ins.induction lt t x <;> intros <;> simp_all! (config := { eta := false }) <;>
     run_tac
@@ -206,31 +225,34 @@ theorem isSearchable_ins [DecidableRel lt] {t x} [IsStrictWeakOrder α lt] :
   · apply is_searchable_balance2_node; assumption; apply ih h_hs₂; simp [*]
     assumption
   · apply ih h_hs₂; assumption; simp [*]
-#align rbnode.is_searchable_ins Rbnode.isSearchable_ins
+#align rbnode.is_searchable_ins Std.RBNode.isSearchableIns
 
 /- ./././Mathport/Syntax/Translate/Tactic/Builtin.lean:69:18: unsupported non-interactive tactic rbnode.is_searchable_tactic -/
-theorem isSearchable_mkInsertResult {c t} :
-    IsSearchable lt t none none → IsSearchable lt (mkInsertResult c t) none none := by
+theorem Std.RBNode.isSearchableMkInsertResult {c t} :
+    Std.RBNode.IsSearchable lt t none none →
+      Std.RBNode.IsSearchable lt (Std.RBNode.mkInsertResult c t) none none :=
+  by
   classical
   cases c <;> cases t <;> simp [mk_insert_result]
   · intro h;
     run_tac
       is_searchable_tactic
-#align rbnode.is_searchable_mk_insert_result Rbnode.isSearchable_mkInsertResult
+#align rbnode.is_searchable_mk_insert_result Std.RBNode.isSearchableMkInsertResult
 
-theorem isSearchable_insert [DecidableRel lt] {t x} [IsStrictWeakOrder α lt] :
-    IsSearchable lt t none none → IsSearchable lt (insert lt t x) none none := by intro h;
-  simp [insert]; apply is_searchable_mk_insert_result;
+theorem Std.RBNode.isSearchableInsert [DecidableRel lt] {t x} [IsStrictWeakOrder α lt] :
+    Std.RBNode.IsSearchable lt t none none →
+      Std.RBNode.IsSearchable lt (Std.RBNode.insert lt t x) none none :=
+  by intro h; simp [insert]; apply is_searchable_mk_insert_result;
   apply is_searchable_ins <;>
     ·
       first
       | assumption
       | simp
-#align rbnode.is_searchable_insert Rbnode.isSearchable_insert
+#align rbnode.is_searchable_insert Std.RBNode.isSearchableInsert
 
-end Rbnode
+end Std.RBNode
 
-namespace Rbnode
+namespace Std.RBNode
 
 section MembershipLemmas
 
@@ -238,80 +260,83 @@ parameter {α : Type u} (lt : α → α → Prop)
 
 attribute [local simp] mem balance1_node balance2_node
 
-local infixl:0 " ∈ " => Mem lt
+local infixl:0 " ∈ " => Std.RBNode.Mem lt
 
-theorem mem_balance1Node_of_mem_left {x s} (v) (t : Rbnode α) :
-    (x ∈ s) → (x ∈ balance1Node s v t) :=
+theorem Std.RBNode.mem_balance1Node_of_mem_left {x s} (v) (t : Std.RBNode α) :
+    (x ∈ s) → (x ∈ Std.RBNode.balance1Node s v t) :=
   by
   cases s <;> simp [false_imp_iff]
   all_goals
     apply balance.cases s_lchild s_val s_rchild <;> intros <;> simp at * <;> cases_type* or.1 <;>
       simp [*]
-#align rbnode.mem_balance1_node_of_mem_left Rbnode.mem_balance1Node_of_mem_left
+#align rbnode.mem_balance1_node_of_mem_left Std.RBNode.mem_balance1Node_of_mem_left
 
-theorem mem_balance2Node_of_mem_left {x s} (v) (t : Rbnode α) :
-    (x ∈ s) → (x ∈ balance2Node s v t) :=
+theorem Std.RBNode.mem_balance2Node_of_mem_left {x s} (v) (t : Std.RBNode α) :
+    (x ∈ s) → (x ∈ Std.RBNode.balance2Node s v t) :=
   by
   cases s <;> simp [false_imp_iff]
   all_goals
     apply balance.cases s_lchild s_val s_rchild <;> intros <;> simp at * <;> cases_type* or.1 <;>
       simp [*]
-#align rbnode.mem_balance2_node_of_mem_left Rbnode.mem_balance2Node_of_mem_left
+#align rbnode.mem_balance2_node_of_mem_left Std.RBNode.mem_balance2Node_of_mem_left
 
-theorem mem_balance1Node_of_mem_right {x t} (v) (s : Rbnode α) :
-    (x ∈ t) → (x ∈ balance1Node s v t) := by
+theorem Std.RBNode.mem_balance1Node_of_mem_right {x t} (v) (s : Std.RBNode α) :
+    (x ∈ t) → (x ∈ Std.RBNode.balance1Node s v t) :=
+  by
   intros; cases s <;> simp [*]
   all_goals apply balance.cases s_lchild s_val s_rchild <;> intros <;> simp [*]
-#align rbnode.mem_balance1_node_of_mem_right Rbnode.mem_balance1Node_of_mem_right
+#align rbnode.mem_balance1_node_of_mem_right Std.RBNode.mem_balance1Node_of_mem_right
 
-theorem mem_balance2Node_of_mem_right {x t} (v) (s : Rbnode α) :
-    (x ∈ t) → (x ∈ balance2Node s v t) := by
+theorem Std.RBNode.mem_balance2Node_of_mem_right {x t} (v) (s : Std.RBNode α) :
+    (x ∈ t) → (x ∈ Std.RBNode.balance2Node s v t) :=
+  by
   intros; cases s <;> simp [*]
   all_goals apply balance.cases s_lchild s_val s_rchild <;> intros <;> simp [*]
-#align rbnode.mem_balance2_node_of_mem_right Rbnode.mem_balance2Node_of_mem_right
+#align rbnode.mem_balance2_node_of_mem_right Std.RBNode.mem_balance2Node_of_mem_right
 
-theorem mem_balance1Node_of_incomp {x v} (s t) :
-    ¬lt x v ∧ ¬lt v x → s ≠ leaf → (x ∈ balance1Node s v t) :=
+theorem Std.RBNode.mem_balance1Node_of_incomp {x v} (s t) :
+    ¬lt x v ∧ ¬lt v x → s ≠ Std.RBNode.nil → (x ∈ Std.RBNode.balance1Node s v t) :=
   by
   intros; cases s <;> simp
   · contradiction
   all_goals apply balance.cases s_lchild s_val s_rchild <;> intros <;> simp [*]
-#align rbnode.mem_balance1_node_of_incomp Rbnode.mem_balance1Node_of_incomp
+#align rbnode.mem_balance1_node_of_incomp Std.RBNode.mem_balance1Node_of_incomp
 
-theorem mem_balance2Node_of_incomp {x v} (s t) :
-    ¬lt v x ∧ ¬lt x v → s ≠ leaf → (x ∈ balance2Node s v t) :=
+theorem Std.RBNode.mem_balance2Node_of_incomp {x v} (s t) :
+    ¬lt v x ∧ ¬lt x v → s ≠ Std.RBNode.nil → (x ∈ Std.RBNode.balance2Node s v t) :=
   by
   intros; cases s <;> simp
   · contradiction
   all_goals apply balance.cases s_lchild s_val s_rchild <;> intros <;> simp [*]
-#align rbnode.mem_balance2_node_of_incomp Rbnode.mem_balance2Node_of_incomp
+#align rbnode.mem_balance2_node_of_incomp Std.RBNode.mem_balance2Node_of_incomp
 
-theorem ins_ne_leaf [DecidableRel lt] (t : Rbnode α) (x : α) : t.ins lt x ≠ leaf :=
-  by
+theorem Std.RBNode.ins_ne_nil [DecidableRel lt] (t : Std.RBNode α) (x : α) :
+    t.ins lt x ≠ Std.RBNode.nil := by
   apply ins.induction lt t x
   any_goals intros; simp [ins, *]
   · intros; apply balance1_node_ne_leaf; assumption
   · intros; apply balance2_node_ne_leaf; assumption
-#align rbnode.ins_ne_leaf Rbnode.ins_ne_leaf
+#align rbnode.ins_ne_leaf Std.RBNode.ins_ne_nil
 
-theorem insert_ne_leaf [DecidableRel lt] (t : Rbnode α) (x : α) : insert lt t x ≠ leaf :=
+theorem Std.RBNode.insert_ne_nil [DecidableRel lt] (t : Std.RBNode α) (x : α) :
+    Std.RBNode.insert lt t x ≠ Std.RBNode.nil :=
   by
   simp [insert]
   cases he : ins lt t x <;> cases get_color t <;> simp [mk_insert_result]
   · have := ins_ne_leaf lt t x; contradiction
   · exact absurd he (ins_ne_leaf _ _ _)
-#align rbnode.insert_ne_leaf Rbnode.insert_ne_leaf
+#align rbnode.insert_ne_leaf Std.RBNode.insert_ne_nil
 
-theorem mem_ins_of_incomp [DecidableRel lt] (t : Rbnode α) {x y : α} :
+theorem Std.RBNode.mem_ins_of_incomp [DecidableRel lt] (t : Std.RBNode α) {x y : α} :
     ∀ h : ¬lt x y ∧ ¬lt y x, x ∈ t.ins lt y :=
   by
   apply ins.induction lt t y <;> intros <;> simp [ins, *]
   · have := ih h; apply mem_balance1_node_of_mem_left; assumption
   · have := ih h; apply mem_balance2_node_of_mem_left; assumption
-#align rbnode.mem_ins_of_incomp Rbnode.mem_ins_of_incomp
+#align rbnode.mem_ins_of_incomp Std.RBNode.mem_ins_of_incomp
 
-theorem mem_ins_of_mem [DecidableRel lt] [IsStrictWeakOrder α lt] {t : Rbnode α} (z : α) :
-    ∀ {x} (h : x ∈ t), x ∈ t.ins lt z :=
+theorem Std.RBNode.mem_ins_of_mem [DecidableRel lt] [IsStrictWeakOrder α lt] {t : Std.RBNode α}
+    (z : α) : ∀ {x} (h : x ∈ t), x ∈ t.ins lt z :=
   by
   apply ins.induction lt t z <;> intros <;> simp_all [ins] <;> try contradiction <;>
     cases_type* or.1
@@ -326,47 +351,51 @@ theorem mem_ins_of_mem [DecidableRel lt] [IsStrictWeakOrder α lt] {t : Rbnode �
   · have := ins_ne_leaf lt a z; apply mem_balance2_node_of_incomp; cases h; simp [*]
     apply ins_ne_leaf
   · apply mem_balance2_node_of_mem_left; apply ih h
-#align rbnode.mem_ins_of_mem Rbnode.mem_ins_of_mem
+#align rbnode.mem_ins_of_mem Std.RBNode.mem_ins_of_mem
 
-theorem mem_mkInsertResult {a t} (c) : Mem lt a t → Mem lt a (mkInsertResult c t) := by
+theorem Std.RBNode.mem_mkInsertResult {a t} (c) :
+    Std.RBNode.Mem lt a t → Std.RBNode.Mem lt a (Std.RBNode.mkInsertResult c t) := by
   intros <;> cases c <;> cases t <;> simp_all [mk_insert_result, mem]
-#align rbnode.mem_mk_insert_result Rbnode.mem_mkInsertResult
+#align rbnode.mem_mk_insert_result Std.RBNode.mem_mkInsertResult
 
-theorem mem_of_mem_mkInsertResult {a t c} : Mem lt a (mkInsertResult c t) → Mem lt a t := by
+theorem Std.RBNode.mem_of_mem_mkInsertResult {a t c} :
+    Std.RBNode.Mem lt a (Std.RBNode.mkInsertResult c t) → Std.RBNode.Mem lt a t := by
   cases t <;> cases c <;> simp [mk_insert_result, mem] <;> intros <;> assumption
-#align rbnode.mem_of_mem_mk_insert_result Rbnode.mem_of_mem_mkInsertResult
+#align rbnode.mem_of_mem_mk_insert_result Std.RBNode.mem_of_mem_mkInsertResult
 
-theorem mem_insert_of_incomp [DecidableRel lt] (t : Rbnode α) {x y : α} :
+theorem Std.RBNode.mem_insert_of_incomp [DecidableRel lt] (t : Std.RBNode α) {x y : α} :
     ∀ h : ¬lt x y ∧ ¬lt y x, x ∈ t.insert lt y := by
   intros <;> unfold insert <;> apply mem_mk_insert_result <;> apply mem_ins_of_incomp <;> assumption
-#align rbnode.mem_insert_of_incomp Rbnode.mem_insert_of_incomp
+#align rbnode.mem_insert_of_incomp Std.RBNode.mem_insert_of_incomp
 
-theorem mem_insert_of_mem [DecidableRel lt] [IsStrictWeakOrder α lt] {t x} (z) :
+#print Std.RBNode.mem_insert_of_mem /-
+theorem Std.RBNode.mem_insert_of_mem [DecidableRel lt] [IsStrictWeakOrder α lt] {t x} (z) :
     (x ∈ t) → (x ∈ t.insert lt z) := by
   intros <;> apply mem_mk_insert_result <;> apply mem_ins_of_mem <;> assumption
-#align rbnode.mem_insert_of_mem Rbnode.mem_insert_of_mem
+#align rbnode.mem_insert_of_mem Std.RBNode.mem_insert_of_mem
+-/
 
-theorem of_mem_balance1Node {x s v t} :
-    (x ∈ balance1Node s v t) → (x ∈ s) ∨ ¬lt x v ∧ ¬lt v x ∨ (x ∈ t) :=
+theorem Std.RBNode.of_mem_balance1Node {x s v t} :
+    (x ∈ Std.RBNode.balance1Node s v t) → (x ∈ s) ∨ ¬lt x v ∧ ¬lt v x ∨ (x ∈ t) :=
   by
   cases s <;> simp
   · intros; simp [*]
   all_goals
     apply balance.cases s_lchild s_val s_rchild <;> intros <;> simp_all <;> cases_type* or.1 <;>
       simp [*]
-#align rbnode.of_mem_balance1_node Rbnode.of_mem_balance1Node
+#align rbnode.of_mem_balance1_node Std.RBNode.of_mem_balance1Node
 
-theorem of_mem_balance2Node {x s v t} :
-    (x ∈ balance2Node s v t) → (x ∈ s) ∨ ¬lt x v ∧ ¬lt v x ∨ (x ∈ t) :=
+theorem Std.RBNode.of_mem_balance2Node {x s v t} :
+    (x ∈ Std.RBNode.balance2Node s v t) → (x ∈ s) ∨ ¬lt x v ∧ ¬lt v x ∨ (x ∈ t) :=
   by
   cases s <;> simp
   · intros; simp [*]
   all_goals
     apply balance.cases s_lchild s_val s_rchild <;> intros <;> simp_all <;> cases_type* or.1 <;>
       simp [*]
-#align rbnode.of_mem_balance2_node Rbnode.of_mem_balance2Node
+#align rbnode.of_mem_balance2_node Std.RBNode.of_mem_balance2Node
 
-theorem equiv_or_mem_of_mem_ins [DecidableRel lt] {t : Rbnode α} {x z} :
+theorem Std.RBNode.equiv_or_mem_of_mem_ins [DecidableRel lt] {t : Std.RBNode α} {x z} :
     ∀ h : x ∈ t.ins lt z, x ≈[lt]z ∨ (x ∈ t) :=
   by
   apply ins.induction lt t z <;> intros <;> simp_all [ins, StrictWeakOrder.Equiv] <;>
@@ -379,38 +408,39 @@ theorem equiv_or_mem_of_mem_ins [DecidableRel lt] {t : Rbnode α} {x z} :
   · have h' := of_mem_balance2_node lt h; cases_type* or.1
     have := ih h'; cases_type* or.1
     all_goals simp [h, *]
-#align rbnode.equiv_or_mem_of_mem_ins Rbnode.equiv_or_mem_of_mem_ins
+#align rbnode.equiv_or_mem_of_mem_ins Std.RBNode.equiv_or_mem_of_mem_ins
 
-theorem equiv_or_mem_of_mem_insert [DecidableRel lt] {t : Rbnode α} {x z} :
+theorem Std.RBNode.equiv_or_mem_of_mem_insert [DecidableRel lt] {t : Std.RBNode α} {x z} :
     ∀ h : x ∈ t.insert lt z, x ≈[lt]z ∨ (x ∈ t) := by simp [insert]; intros;
   apply equiv_or_mem_of_mem_ins; exact mem_of_mem_mk_insert_result lt h
-#align rbnode.equiv_or_mem_of_mem_insert Rbnode.equiv_or_mem_of_mem_insert
+#align rbnode.equiv_or_mem_of_mem_insert Std.RBNode.equiv_or_mem_of_mem_insert
 
 attribute [local simp] mem_exact
 
-theorem memExact_balance1Node_of_memExact {x s} (v) (t : Rbnode α) :
-    MemExact x s → MemExact x (balance1Node s v t) :=
+theorem Std.RBNode.memExact_balance1Node_of_memExact {x s} (v) (t : Std.RBNode α) :
+    Std.RBNode.MemExact x s → Std.RBNode.MemExact x (Std.RBNode.balance1Node s v t) :=
   by
   cases s <;> simp [false_imp_iff]
   all_goals
     apply balance.cases s_lchild s_val s_rchild <;> intros <;> simp_all <;> cases_type* or.1 <;>
       simp [*]
-#align rbnode.mem_exact_balance1_node_of_mem_exact Rbnode.memExact_balance1Node_of_memExact
+#align rbnode.mem_exact_balance1_node_of_mem_exact Std.RBNode.memExact_balance1Node_of_memExact
 
-theorem memExact_balance2Node_of_memExact {x s} (v) (t : Rbnode α) :
-    MemExact x s → MemExact x (balance2Node s v t) :=
+theorem Std.RBNode.memExact_balance2Node_of_memExact {x s} (v) (t : Std.RBNode α) :
+    Std.RBNode.MemExact x s → Std.RBNode.MemExact x (Std.RBNode.balance2Node s v t) :=
   by
   cases s <;> simp [false_imp_iff]
   all_goals
     apply balance.cases s_lchild s_val s_rchild <;> intros <;> simp_all <;> cases_type* or.1 <;>
       simp [*]
-#align rbnode.mem_exact_balance2_node_of_mem_exact Rbnode.memExact_balance2Node_of_memExact
+#align rbnode.mem_exact_balance2_node_of_mem_exact Std.RBNode.memExact_balance2Node_of_memExact
 
-theorem find_balance1Node [DecidableRel lt] [IsStrictWeakOrder α lt] {x y z t s} :
+theorem Std.RBNode.find?_balance1Node [DecidableRel lt] [IsStrictWeakOrder α lt] {x y z t s} :
     ∀ {lo hi},
-      IsSearchable lt t lo (some z) →
-        IsSearchable lt s (some z) hi →
-          find lt t y = some x → y ≈[lt]x → find lt (balance1Node t z s) y = some x :=
+      Std.RBNode.IsSearchable lt t lo (some z) →
+        Std.RBNode.IsSearchable lt s (some z) hi →
+          Std.RBNode.find? lt t y = some x →
+            y ≈[lt]x → Std.RBNode.find? lt (Std.RBNode.balance1Node t z s) y = some x :=
   by
   intro _ _ hs₁ hs₂ heq heqv
   have hs := is_searchable_balance1_node lt hs₁ hs₂
@@ -419,13 +449,15 @@ theorem find_balance1Node [DecidableRel lt] [IsStrictWeakOrder α lt] {x y z t s
   have := mem_exact_balance1_node_of_mem_exact z s this
   have := Iff.mp (find_correct_exact hs) this
   exact Eq.trans (find_eq_find_of_eqv hs heqv) this
-#align rbnode.find_balance1_node Rbnode.find_balance1Node
+#align rbnode.find_balance1_node Std.RBNode.find?_balance1Node
 
-theorem find_balance2Node [DecidableRel lt] [IsStrictWeakOrder α lt] {x y z s t} [IsTrans α lt] :
+theorem Std.RBNode.find?_balance2Node [DecidableRel lt] [IsStrictWeakOrder α lt] {x y z s t}
+    [IsTrans α lt] :
     ∀ {lo hi},
-      IsSearchable lt s lo (some z) →
-        IsSearchable lt t (some z) hi →
-          find lt t y = some x → y ≈[lt]x → find lt (balance2Node t z s) y = some x :=
+      Std.RBNode.IsSearchable lt s lo (some z) →
+        Std.RBNode.IsSearchable lt t (some z) hi →
+          Std.RBNode.find? lt t y = some x →
+            y ≈[lt]x → Std.RBNode.find? lt (Std.RBNode.balance2Node t z s) y = some x :=
   by
   intro _ _ hs₁ hs₂ heq heqv
   have hs := is_searchable_balance2_node lt hs₁ hs₂
@@ -434,12 +466,12 @@ theorem find_balance2Node [DecidableRel lt] [IsStrictWeakOrder α lt] {x y z s t
   have := mem_exact_balance2_node_of_mem_exact z s this
   have := Iff.mp (find_correct_exact hs) this
   exact Eq.trans (find_eq_find_of_eqv hs heqv) this
-#align rbnode.find_balance2_node Rbnode.find_balance2Node
+#align rbnode.find_balance2_node Std.RBNode.find?_balance2Node
 
 -- Auxiliary lemma
-theorem ite_eq_of_not_lt [DecidableRel lt] [IsStrictOrder α lt] {a b} {β : Type v} (t s : β)
-    (h : lt b a) : (if lt a b then t else s) = s := by have := not_lt_of_lt h; simp [*]
-#align rbnode.ite_eq_of_not_lt Rbnode.ite_eq_of_not_lt
+theorem Std.RBNode.ite_eq_of_not_lt [DecidableRel lt] [IsStrictOrder α lt] {a b} {β : Type v}
+    (t s : β) (h : lt b a) : (if lt a b then t else s) = s := by have := not_lt_of_lt h; simp [*]
+#align rbnode.ite_eq_of_not_lt Std.RBNode.ite_eq_of_not_lt
 
 attribute [local simp] ite_eq_of_not_lt
 
@@ -456,10 +488,11 @@ private unsafe def simp_fi : tactic Unit :=
 /- ./././Mathport/Syntax/Translate/Tactic/Builtin.lean:69:18: unsupported non-interactive tactic _private.3968712505.simp_fi -/
 /- ./././Mathport/Syntax/Translate/Tactic/Builtin.lean:69:18: unsupported non-interactive tactic _private.3968712505.simp_fi -/
 /- ./././Mathport/Syntax/Translate/Tactic/Builtin.lean:69:18: unsupported non-interactive tactic _private.3968712505.simp_fi -/
-theorem find_ins_of_eqv [DecidableRel lt] [IsStrictWeakOrder α lt] {x y : α} {t : Rbnode α}
-    (he : x ≈[lt]y) :
-    ∀ {lo hi} (hs : IsSearchable lt t lo hi) (hlt₁ : Lift lt lo (some x))
-      (hlt₂ : Lift lt (some x) hi), find lt (ins lt t x) y = some x :=
+theorem Std.RBNode.find?_ins_of_eqv [DecidableRel lt] [IsStrictWeakOrder α lt] {x y : α}
+    {t : Std.RBNode α} (he : x ≈[lt]y) :
+    ∀ {lo hi} (hs : Std.RBNode.IsSearchable lt t lo hi) (hlt₁ : Std.RBNode.Lift lt lo (some x))
+      (hlt₂ : Std.RBNode.Lift lt (some x) hi),
+      Std.RBNode.find? lt (Std.RBNode.ins lt t x) y = some x :=
   by
   simp [StrictWeakOrder.Equiv] at he 
   apply ins.induction lt t x <;> intros
@@ -497,24 +530,26 @@ theorem find_ins_of_eqv [DecidableRel lt] [IsStrictWeakOrder α lt] {x y : α} {
     have := ih hs_hs₂ hc hlt₂
     run_tac
       simp_fi
-#align rbnode.find_ins_of_eqv Rbnode.find_ins_of_eqv
+#align rbnode.find_ins_of_eqv Std.RBNode.find?_ins_of_eqv
 
-theorem find_mkInsertResult [DecidableRel lt] (c : Color) (t : Rbnode α) (x : α) :
-    find lt (mkInsertResult c t) x = find lt t x :=
+theorem Std.RBNode.find?_mkInsertResult [DecidableRel lt] (c : RBColor) (t : Std.RBNode α) (x : α) :
+    Std.RBNode.find? lt (Std.RBNode.mkInsertResult c t) x = Std.RBNode.find? lt t x :=
   by
   cases t <;> cases c <;> simp [mk_insert_result]
   · simp [find]; cases cmpUsing lt x t_val <;> simp [find]
-#align rbnode.find_mk_insert_result Rbnode.find_mkInsertResult
+#align rbnode.find_mk_insert_result Std.RBNode.find?_mkInsertResult
 
-theorem find_insert_of_eqv [DecidableRel lt] [IsStrictWeakOrder α lt] {x y : α} {t : Rbnode α}
-    (he : x ≈[lt]y) : IsSearchable lt t none none → find lt (insert lt t x) y = some x :=
+theorem Std.RBNode.find?_insert_of_eqv [DecidableRel lt] [IsStrictWeakOrder α lt] {x y : α}
+    {t : Std.RBNode α} (he : x ≈[lt]y) :
+    Std.RBNode.IsSearchable lt t none none →
+      Std.RBNode.find? lt (Std.RBNode.insert lt t x) y = some x :=
   by
   intro hs
   simp [insert, find_mk_insert_result]
   apply find_ins_of_eqv lt he hs <;> simp
-#align rbnode.find_insert_of_eqv Rbnode.find_insert_of_eqv
+#align rbnode.find_insert_of_eqv Std.RBNode.find?_insert_of_eqv
 
-theorem weak_trichotomous (x y) {p : Prop} (is_lt : ∀ h : lt x y, p)
+theorem Std.RBNode.weak_trichotomous (x y) {p : Prop} (is_lt : ∀ h : lt x y, p)
     (is_eqv : ∀ h : ¬lt x y ∧ ¬lt y x, p) (is_gt : ∀ h : lt y x, p) : p :=
   by
   by_cases lt x y
@@ -522,28 +557,30 @@ theorem weak_trichotomous (x y) {p : Prop} (is_lt : ∀ h : lt x y, p)
   by_cases lt y x
   · apply is_gt; assumption
   · apply is_eqv; constructor <;> assumption
-#align rbnode.weak_trichotomous Rbnode.weak_trichotomous
+#align rbnode.weak_trichotomous Std.RBNode.weak_trichotomous
 
 section FindInsOfNotEqv
 
 section SimpAuxLemmas
 
-theorem find_black_eq_find_red [DecidableRel lt] {l y r x} :
-    find lt (black_node l y r) x = find lt (red_node l y r) x := by simp [find];
-  all_goals cases cmpUsing lt x y <;> simp [find]
-#align rbnode.find_black_eq_find_red Rbnode.find_black_eq_find_red
+theorem Std.RBNode.find?_black_eq_find?_red [DecidableRel lt] {l y r x} :
+    Std.RBNode.find? lt (black_node l y r) x = Std.RBNode.find? lt (Std.RBNode.node l y r) x := by
+  simp [find]; all_goals cases cmpUsing lt x y <;> simp [find]
+#align rbnode.find_black_eq_find_red Std.RBNode.find?_black_eq_find?_red
 
-theorem find_red_of_lt [DecidableRel lt] {l y r x} (h : lt x y) :
-    find lt (red_node l y r) x = find lt l x := by simp [find, cmpUsing, *]
-#align rbnode.find_red_of_lt Rbnode.find_red_of_lt
+theorem Std.RBNode.find?_red_of_lt [DecidableRel lt] {l y r x} (h : lt x y) :
+    Std.RBNode.find? lt (Std.RBNode.node l y r) x = Std.RBNode.find? lt l x := by
+  simp [find, cmpUsing, *]
+#align rbnode.find_red_of_lt Std.RBNode.find?_red_of_lt
 
-theorem find_red_of_gt [DecidableRel lt] [IsStrictOrder α lt] {l y r x} (h : lt y x) :
-    find lt (red_node l y r) x = find lt r x := by have := not_lt_of_lt h; simp [find, cmpUsing, *]
-#align rbnode.find_red_of_gt Rbnode.find_red_of_gt
+theorem Std.RBNode.find?_red_of_gt [DecidableRel lt] [IsStrictOrder α lt] {l y r x} (h : lt y x) :
+    Std.RBNode.find? lt (Std.RBNode.node l y r) x = Std.RBNode.find? lt r x := by
+  have := not_lt_of_lt h; simp [find, cmpUsing, *]
+#align rbnode.find_red_of_gt Std.RBNode.find?_red_of_gt
 
-theorem find_red_of_incomp [DecidableRel lt] {l y r x} (h : ¬lt x y ∧ ¬lt y x) :
-    find lt (red_node l y r) x = some y := by simp [find, cmpUsing, *]
-#align rbnode.find_red_of_incomp Rbnode.find_red_of_incomp
+theorem Std.RBNode.find?_red_of_incomp [DecidableRel lt] {l y r x} (h : ¬lt x y ∧ ¬lt y x) :
+    Std.RBNode.find? lt (Std.RBNode.node l y r) x = some y := by simp [find, cmpUsing, *]
+#align rbnode.find_red_of_incomp Std.RBNode.find?_red_of_incomp
 
 end SimpAuxLemmas
 
@@ -553,9 +590,12 @@ attribute [local simp] find_black_eq_find_red find_red_of_lt find_red_of_lt find
 variable [IsStrictWeakOrder α lt] [DecidableRel lt]
 
 /- ./././Mathport/Syntax/Translate/Tactic/Builtin.lean:69:18: unsupported non-interactive tactic rbnode.is_searchable_tactic -/
-theorem find_balance1_lt {l r t v x y lo hi} (h : lt x y) (hl : IsSearchable lt l lo (some v))
-    (hr : IsSearchable lt r (some v) (some y)) (ht : IsSearchable lt t (some y) hi) :
-    find lt (balance1 l v r y t) x = find lt (red_node l v r) x :=
+theorem Std.RBNode.find?_balance1_lt {l r t v x y lo hi} (h : lt x y)
+    (hl : Std.RBNode.IsSearchable lt l lo (some v))
+    (hr : Std.RBNode.IsSearchable lt r (some v) (some y))
+    (ht : Std.RBNode.IsSearchable lt t (some y) hi) :
+    Std.RBNode.find? lt (Std.RBNode.balance1 l v r y t) x =
+      Std.RBNode.find? lt (Std.RBNode.node l v r) x :=
   by
   revert hl hr ht;
   apply balance.cases l v r <;> intros <;> simp [*] <;>
@@ -566,7 +606,7 @@ theorem find_balance1_lt {l r t v x y lo hi} (h : lt x y) (hl : IsSearchable lt 
     · have := trans_of lt (lo_lt_hi hr_hs₁) h'; simp [*]
     · have : lt y_1 x := lt_of_lt_of_incomp (lo_lt_hi hr_hs₁) h'; simp [*]
     · apply weak_trichotomous lt y_1 x <;> intros <;> simp [*]
-#align rbnode.find_balance1_lt Rbnode.find_balance1_lt
+#align rbnode.find_balance1_lt Std.RBNode.find?_balance1_lt
 
 /- ./././Mathport/Syntax/Translate/Expr.lean:336:4: warning: unsupported (TODO): `[tacs] -/
 unsafe def ins_ne_leaf_tac :=
@@ -575,12 +615,12 @@ unsafe def ins_ne_leaf_tac :=
 
 /- ./././Mathport/Syntax/Translate/Tactic/Builtin.lean:69:18: unsupported non-interactive tactic rbnode.is_searchable_tactic -/
 /- ./././Mathport/Syntax/Translate/Tactic/Builtin.lean:69:18: unsupported non-interactive tactic ins_ne_leaf_tac -/
-theorem find_balance1Node_lt {t s x y lo hi} (hlt : lt y x) (ht : IsSearchable lt t lo (some x))
-    (hs : IsSearchable lt s (some x) hi)
-    (hne : t ≠ leaf := by
+theorem Std.RBNode.find?_balance1Node_lt {t s x y lo hi} (hlt : lt y x)
+    (ht : Std.RBNode.IsSearchable lt t lo (some x)) (hs : Std.RBNode.IsSearchable lt s (some x) hi)
+    (hne : t ≠ Std.RBNode.nil := by
       run_tac
         ins_ne_leaf_tac) :
-    find lt (balance1Node t x s) y = find lt t y :=
+    Std.RBNode.find? lt (Std.RBNode.balance1Node t x s) y = Std.RBNode.find? lt t y :=
   by
   cases t <;> simp [balance1_node]
   · contradiction
@@ -588,12 +628,14 @@ theorem find_balance1Node_lt {t s x y lo hi} (hlt : lt y x) (ht : IsSearchable l
     run_tac
       is_searchable_tactic;
     apply find_balance1_lt; assumption'
-#align rbnode.find_balance1_node_lt Rbnode.find_balance1Node_lt
+#align rbnode.find_balance1_node_lt Std.RBNode.find?_balance1Node_lt
 
 /- ./././Mathport/Syntax/Translate/Tactic/Builtin.lean:69:18: unsupported non-interactive tactic rbnode.is_searchable_tactic -/
-theorem find_balance1_gt {l r t v x y lo hi} (h : lt y x) (hl : IsSearchable lt l lo (some v))
-    (hr : IsSearchable lt r (some v) (some y)) (ht : IsSearchable lt t (some y) hi) :
-    find lt (balance1 l v r y t) x = find lt t x :=
+theorem Std.RBNode.find?_balance1_gt {l r t v x y lo hi} (h : lt y x)
+    (hl : Std.RBNode.IsSearchable lt l lo (some v))
+    (hr : Std.RBNode.IsSearchable lt r (some v) (some y))
+    (ht : Std.RBNode.IsSearchable lt t (some y) hi) :
+    Std.RBNode.find? lt (Std.RBNode.balance1 l v r y t) x = Std.RBNode.find? lt t x :=
   by
   revert hl hr ht;
   apply balance.cases l v r <;> intros <;> simp [*] <;>
@@ -601,28 +643,30 @@ theorem find_balance1_gt {l r t v x y lo hi} (h : lt y x) (hl : IsSearchable lt 
       is_searchable_tactic
   · have := trans_of lt (lo_lt_hi hr) h; simp [*]
   · have := trans_of lt (lo_lt_hi hr_hs₂) h; simp [*]
-#align rbnode.find_balance1_gt Rbnode.find_balance1_gt
+#align rbnode.find_balance1_gt Std.RBNode.find?_balance1_gt
 
 /- ./././Mathport/Syntax/Translate/Tactic/Builtin.lean:69:18: unsupported non-interactive tactic rbnode.is_searchable_tactic -/
 /- ./././Mathport/Syntax/Translate/Tactic/Builtin.lean:69:18: unsupported non-interactive tactic ins_ne_leaf_tac -/
-theorem find_balance1Node_gt {t s x y lo hi} (h : lt x y) (ht : IsSearchable lt t lo (some x))
-    (hs : IsSearchable lt s (some x) hi)
-    (hne : t ≠ leaf := by
+theorem Std.RBNode.find?_balance1Node_gt {t s x y lo hi} (h : lt x y)
+    (ht : Std.RBNode.IsSearchable lt t lo (some x)) (hs : Std.RBNode.IsSearchable lt s (some x) hi)
+    (hne : t ≠ Std.RBNode.nil := by
       run_tac
         ins_ne_leaf_tac) :
-    find lt (balance1Node t x s) y = find lt s y :=
+    Std.RBNode.find? lt (Std.RBNode.balance1Node t x s) y = Std.RBNode.find? lt s y :=
   by
   cases t <;> simp [balance1_node]
   all_goals intros;
     run_tac
       is_searchable_tactic;
     apply find_balance1_gt; assumption'
-#align rbnode.find_balance1_node_gt Rbnode.find_balance1Node_gt
+#align rbnode.find_balance1_node_gt Std.RBNode.find?_balance1Node_gt
 
 /- ./././Mathport/Syntax/Translate/Tactic/Builtin.lean:69:18: unsupported non-interactive tactic rbnode.is_searchable_tactic -/
-theorem find_balance1_eqv {l r t v x y lo hi} (h : ¬lt x y ∧ ¬lt y x)
-    (hl : IsSearchable lt l lo (some v)) (hr : IsSearchable lt r (some v) (some y))
-    (ht : IsSearchable lt t (some y) hi) : find lt (balance1 l v r y t) x = some y :=
+theorem Std.RBNode.find?_balance1_eqv {l r t v x y lo hi} (h : ¬lt x y ∧ ¬lt y x)
+    (hl : Std.RBNode.IsSearchable lt l lo (some v))
+    (hr : Std.RBNode.IsSearchable lt r (some v) (some y))
+    (ht : Std.RBNode.IsSearchable lt t (some y) hi) :
+    Std.RBNode.find? lt (Std.RBNode.balance1 l v r y t) x = some y :=
   by
   revert hl hr ht;
   apply balance.cases l v r <;> intros <;> simp [*] <;>
@@ -632,16 +676,16 @@ theorem find_balance1_eqv {l r t v x y lo hi} (h : ¬lt x y ∧ ¬lt y x)
     simp [*]
   · have : lt x_1 x := lt_of_lt_of_incomp (lo_lt_hi hr_hs₂) h.swap
     simp [*]
-#align rbnode.find_balance1_eqv Rbnode.find_balance1_eqv
+#align rbnode.find_balance1_eqv Std.RBNode.find?_balance1_eqv
 
 /- ./././Mathport/Syntax/Translate/Tactic/Builtin.lean:69:18: unsupported non-interactive tactic rbnode.is_searchable_tactic -/
 /- ./././Mathport/Syntax/Translate/Tactic/Builtin.lean:69:18: unsupported non-interactive tactic ins_ne_leaf_tac -/
-theorem find_balance1Node_eqv {t s x y lo hi} (h : ¬lt x y ∧ ¬lt y x)
-    (ht : IsSearchable lt t lo (some y)) (hs : IsSearchable lt s (some y) hi)
-    (hne : t ≠ leaf := by
+theorem Std.RBNode.find?_balance1Node_eqv {t s x y lo hi} (h : ¬lt x y ∧ ¬lt y x)
+    (ht : Std.RBNode.IsSearchable lt t lo (some y)) (hs : Std.RBNode.IsSearchable lt s (some y) hi)
+    (hne : t ≠ Std.RBNode.nil := by
       run_tac
         ins_ne_leaf_tac) :
-    find lt (balance1Node t y s) x = some y :=
+    Std.RBNode.find? lt (Std.RBNode.balance1Node t y s) x = some y :=
   by
   cases t <;> simp [balance1_node]
   · contradiction
@@ -649,12 +693,14 @@ theorem find_balance1Node_eqv {t s x y lo hi} (h : ¬lt x y ∧ ¬lt y x)
     run_tac
       is_searchable_tactic;
     apply find_balance1_eqv; assumption'
-#align rbnode.find_balance1_node_eqv Rbnode.find_balance1Node_eqv
+#align rbnode.find_balance1_node_eqv Std.RBNode.find?_balance1Node_eqv
 
 /- ./././Mathport/Syntax/Translate/Tactic/Builtin.lean:69:18: unsupported non-interactive tactic rbnode.is_searchable_tactic -/
-theorem find_balance2_lt {l v r t x y lo hi} (h : lt x y) (hl : IsSearchable lt l (some y) (some v))
-    (hr : IsSearchable lt r (some v) hi) (ht : IsSearchable lt t lo (some y)) :
-    find lt (balance2 l v r y t) x = find lt t x :=
+theorem Std.RBNode.find?_balance2_lt {l v r t x y lo hi} (h : lt x y)
+    (hl : Std.RBNode.IsSearchable lt l (some y) (some v))
+    (hr : Std.RBNode.IsSearchable lt r (some v) hi)
+    (ht : Std.RBNode.IsSearchable lt t lo (some y)) :
+    Std.RBNode.find? lt (Std.RBNode.balance2 l v r y t) x = Std.RBNode.find? lt t x :=
   by
   revert hl hr ht;
   apply balance.cases l v r <;> intros <;> simp [*] <;>
@@ -662,28 +708,31 @@ theorem find_balance2_lt {l v r t x y lo hi} (h : lt x y) (hl : IsSearchable lt 
       is_searchable_tactic
   · have := trans h (lo_lt_hi hl_hs₁); simp [*]
   · have := trans h (lo_lt_hi hl); simp [*]
-#align rbnode.find_balance2_lt Rbnode.find_balance2_lt
+#align rbnode.find_balance2_lt Std.RBNode.find?_balance2_lt
 
 /- ./././Mathport/Syntax/Translate/Tactic/Builtin.lean:69:18: unsupported non-interactive tactic rbnode.is_searchable_tactic -/
 /- ./././Mathport/Syntax/Translate/Tactic/Builtin.lean:69:18: unsupported non-interactive tactic ins_ne_leaf_tac -/
-theorem find_balance2Node_lt {s t x y lo hi} (h : lt x y) (ht : IsSearchable lt t (some y) hi)
-    (hs : IsSearchable lt s lo (some y))
-    (hne : t ≠ leaf := by
+theorem Std.RBNode.find?_balance2Node_lt {s t x y lo hi} (h : lt x y)
+    (ht : Std.RBNode.IsSearchable lt t (some y) hi) (hs : Std.RBNode.IsSearchable lt s lo (some y))
+    (hne : t ≠ Std.RBNode.nil := by
       run_tac
         ins_ne_leaf_tac) :
-    find lt (balance2Node t y s) x = find lt s x :=
+    Std.RBNode.find? lt (Std.RBNode.balance2Node t y s) x = Std.RBNode.find? lt s x :=
   by
   cases t <;> simp [balance2_node]
   all_goals intros;
     run_tac
       is_searchable_tactic;
     apply find_balance2_lt; assumption'
-#align rbnode.find_balance2_node_lt Rbnode.find_balance2Node_lt
+#align rbnode.find_balance2_node_lt Std.RBNode.find?_balance2Node_lt
 
 /- ./././Mathport/Syntax/Translate/Tactic/Builtin.lean:69:18: unsupported non-interactive tactic rbnode.is_searchable_tactic -/
-theorem find_balance2_gt {l v r t x y lo hi} (h : lt y x) (hl : IsSearchable lt l (some y) (some v))
-    (hr : IsSearchable lt r (some v) hi) (ht : IsSearchable lt t lo (some y)) :
-    find lt (balance2 l v r y t) x = find lt (red_node l v r) x :=
+theorem Std.RBNode.find?_balance2_gt {l v r t x y lo hi} (h : lt y x)
+    (hl : Std.RBNode.IsSearchable lt l (some y) (some v))
+    (hr : Std.RBNode.IsSearchable lt r (some v) hi)
+    (ht : Std.RBNode.IsSearchable lt t lo (some y)) :
+    Std.RBNode.find? lt (Std.RBNode.balance2 l v r y t) x =
+      Std.RBNode.find? lt (Std.RBNode.node l v r) x :=
   by
   revert hl hr ht;
   apply balance.cases l v r <;> intros <;> simp [*] <;>
@@ -694,16 +743,16 @@ theorem find_balance2_gt {l v r t x y lo hi} (h : lt y x) (hl : IsSearchable lt 
     · have : lt x _ := lt_of_incomp_of_lt h'.swap (lo_lt_hi hl_hs₂); simp [*]
     · have := trans h' (lo_lt_hi hl_hs₂); simp [*]
   · apply weak_trichotomous lt y_1 x <;> intros <;> simp [*]
-#align rbnode.find_balance2_gt Rbnode.find_balance2_gt
+#align rbnode.find_balance2_gt Std.RBNode.find?_balance2_gt
 
 /- ./././Mathport/Syntax/Translate/Tactic/Builtin.lean:69:18: unsupported non-interactive tactic rbnode.is_searchable_tactic -/
 /- ./././Mathport/Syntax/Translate/Tactic/Builtin.lean:69:18: unsupported non-interactive tactic ins_ne_leaf_tac -/
-theorem find_balance2Node_gt {s t x y lo hi} (h : lt y x) (ht : IsSearchable lt t (some y) hi)
-    (hs : IsSearchable lt s lo (some y))
-    (hne : t ≠ leaf := by
+theorem Std.RBNode.find?_balance2Node_gt {s t x y lo hi} (h : lt y x)
+    (ht : Std.RBNode.IsSearchable lt t (some y) hi) (hs : Std.RBNode.IsSearchable lt s lo (some y))
+    (hne : t ≠ Std.RBNode.nil := by
       run_tac
         ins_ne_leaf_tac) :
-    find lt (balance2Node t y s) x = find lt t x :=
+    Std.RBNode.find? lt (Std.RBNode.balance2Node t y s) x = Std.RBNode.find? lt t x :=
   by
   cases t <;> simp [balance2_node]
   · contradiction
@@ -711,12 +760,14 @@ theorem find_balance2Node_gt {s t x y lo hi} (h : lt y x) (ht : IsSearchable lt 
     run_tac
       is_searchable_tactic;
     apply find_balance2_gt; assumption'
-#align rbnode.find_balance2_node_gt Rbnode.find_balance2Node_gt
+#align rbnode.find_balance2_node_gt Std.RBNode.find?_balance2Node_gt
 
 /- ./././Mathport/Syntax/Translate/Tactic/Builtin.lean:69:18: unsupported non-interactive tactic rbnode.is_searchable_tactic -/
-theorem find_balance2_eqv {l v r t x y lo hi} (h : ¬lt x y ∧ ¬lt y x)
-    (hl : IsSearchable lt l (some y) (some v)) (hr : IsSearchable lt r (some v) hi)
-    (ht : IsSearchable lt t lo (some y)) : find lt (balance2 l v r y t) x = some y :=
+theorem Std.RBNode.find?_balance2_eqv {l v r t x y lo hi} (h : ¬lt x y ∧ ¬lt y x)
+    (hl : Std.RBNode.IsSearchable lt l (some y) (some v))
+    (hr : Std.RBNode.IsSearchable lt r (some v) hi)
+    (ht : Std.RBNode.IsSearchable lt t lo (some y)) :
+    Std.RBNode.find? lt (Std.RBNode.balance2 l v r y t) x = some y :=
   by
   revert hl hr ht;
   apply balance.cases l v r <;> intros <;> simp [*] <;>
@@ -724,16 +775,16 @@ theorem find_balance2_eqv {l v r t x y lo hi} (h : ¬lt x y ∧ ¬lt y x)
       is_searchable_tactic
   · have := lt_of_incomp_of_lt h (lo_lt_hi hl_hs₁); simp [*]
   · have := lt_of_incomp_of_lt h (lo_lt_hi hl); simp [*]
-#align rbnode.find_balance2_eqv Rbnode.find_balance2_eqv
+#align rbnode.find_balance2_eqv Std.RBNode.find?_balance2_eqv
 
 /- ./././Mathport/Syntax/Translate/Tactic/Builtin.lean:69:18: unsupported non-interactive tactic rbnode.is_searchable_tactic -/
 /- ./././Mathport/Syntax/Translate/Tactic/Builtin.lean:69:18: unsupported non-interactive tactic ins_ne_leaf_tac -/
-theorem find_balance2Node_eqv {t s x y lo hi} (h : ¬lt x y ∧ ¬lt y x)
-    (ht : IsSearchable lt t (some y) hi) (hs : IsSearchable lt s lo (some y))
-    (hne : t ≠ leaf := by
+theorem Std.RBNode.find?_balance2Node_eqv {t s x y lo hi} (h : ¬lt x y ∧ ¬lt y x)
+    (ht : Std.RBNode.IsSearchable lt t (some y) hi) (hs : Std.RBNode.IsSearchable lt s lo (some y))
+    (hne : t ≠ Std.RBNode.nil := by
       run_tac
         ins_ne_leaf_tac) :
-    find lt (balance2Node t y s) x = some y :=
+    Std.RBNode.find? lt (Std.RBNode.balance2Node t y s) x = some y :=
   by
   cases t <;> simp [balance2_node]
   · contradiction
@@ -741,7 +792,7 @@ theorem find_balance2Node_eqv {t s x y lo hi} (h : ¬lt x y ∧ ¬lt y x)
     run_tac
       is_searchable_tactic;
     apply find_balance2_eqv; assumption'
-#align rbnode.find_balance2_node_eqv Rbnode.find_balance2Node_eqv
+#align rbnode.find_balance2_node_eqv Std.RBNode.find?_balance2Node_eqv
 
 /- ./././Mathport/Syntax/Translate/Tactic/Builtin.lean:69:18: unsupported non-interactive tactic _private.3968712505.simp_fi -/
 /- ./././Mathport/Syntax/Translate/Tactic/Builtin.lean:69:18: unsupported non-interactive tactic _private.3968712505.simp_fi -/
@@ -761,9 +812,10 @@ theorem find_balance2Node_eqv {t s x y lo hi} (h : ¬lt x y ∧ ¬lt y x)
 /- ./././Mathport/Syntax/Translate/Tactic/Builtin.lean:69:18: unsupported non-interactive tactic _private.3968712505.simp_fi -/
 /- ./././Mathport/Syntax/Translate/Tactic/Builtin.lean:69:18: unsupported non-interactive tactic _private.3968712505.simp_fi -/
 /- ./././Mathport/Syntax/Translate/Tactic/Builtin.lean:69:18: unsupported non-interactive tactic _private.3968712505.simp_fi -/
-theorem find_ins_of_disj {x y : α} {t : Rbnode α} (hn : lt x y ∨ lt y x) :
-    ∀ {lo hi} (hs : IsSearchable lt t lo hi) (hlt₁ : Lift lt lo (some x))
-      (hlt₂ : Lift lt (some x) hi), find lt (ins lt t x) y = find lt t y :=
+theorem Std.RBNode.find?_ins_of_disj {x y : α} {t : Std.RBNode α} (hn : lt x y ∨ lt y x) :
+    ∀ {lo hi} (hs : Std.RBNode.IsSearchable lt t lo hi) (hlt₁ : Std.RBNode.Lift lt lo (some x))
+      (hlt₂ : Std.RBNode.Lift lt (some x) hi),
+      Std.RBNode.find? lt (Std.RBNode.ins lt t x) y = Std.RBNode.find? lt t y :=
   by
   apply ins.induction lt t x <;> intros
   · cases hn
@@ -842,21 +894,24 @@ theorem find_ins_of_disj {x y : α} {t : Rbnode α} (hn : lt x y ∨ lt y x) :
   · have ih := ih hs_hs₂ hc hlt₂
     run_tac
       simp_fi
-#align rbnode.find_ins_of_disj Rbnode.find_ins_of_disj
+#align rbnode.find_ins_of_disj Std.RBNode.find?_ins_of_disj
 
 end FindInsOfNotEqv
 
-theorem find_insert_of_disj [DecidableRel lt] [IsStrictWeakOrder α lt] {x y : α} {t : Rbnode α}
-    (hd : lt x y ∨ lt y x) :
-    IsSearchable lt t none none → find lt (insert lt t x) y = find lt t y :=
+theorem Std.RBNode.find?_insert_of_disj [DecidableRel lt] [IsStrictWeakOrder α lt] {x y : α}
+    {t : Std.RBNode α} (hd : lt x y ∨ lt y x) :
+    Std.RBNode.IsSearchable lt t none none →
+      Std.RBNode.find? lt (Std.RBNode.insert lt t x) y = Std.RBNode.find? lt t y :=
   by
   intro hs
   simp [insert, find_mk_insert_result]
   apply find_ins_of_disj lt hd hs <;> simp
-#align rbnode.find_insert_of_disj Rbnode.find_insert_of_disj
+#align rbnode.find_insert_of_disj Std.RBNode.find?_insert_of_disj
 
-theorem find_insert_of_not_eqv [DecidableRel lt] [IsStrictWeakOrder α lt] {x y : α} {t : Rbnode α}
-    (hn : ¬x ≈[lt]y) : IsSearchable lt t none none → find lt (insert lt t x) y = find lt t y :=
+theorem Std.RBNode.find?_insert_of_not_eqv [DecidableRel lt] [IsStrictWeakOrder α lt] {x y : α}
+    {t : Std.RBNode α} (hn : ¬x ≈[lt]y) :
+    Std.RBNode.IsSearchable lt t none none →
+      Std.RBNode.find? lt (Std.RBNode.insert lt t x) y = Std.RBNode.find? lt t y :=
   by
   intro hs
   simp [insert, find_mk_insert_result]
@@ -865,7 +920,7 @@ theorem find_insert_of_not_eqv [DecidableRel lt] [IsStrictWeakOrder α lt] {x y 
     simp [StrictWeakOrder.Equiv, Decidable.not_and_iff_or_not, Decidable.not_not_iff] at hn 
     assumption
   apply find_ins_of_disj lt he hs <;> simp
-#align rbnode.find_insert_of_not_eqv Rbnode.find_insert_of_not_eqv
+#align rbnode.find_insert_of_not_eqv Std.RBNode.find?_insert_of_not_eqv
 
 end MembershipLemmas
 
@@ -875,62 +930,73 @@ variable {α : Type u}
 
 open Nat Color
 
-inductive IsBadRedBlack : Rbnode α → Nat → Prop
+inductive Std.RBNode.IsBadRedBlack : Std.RBNode α → Nat → Prop
   |
-  bad_red {c₁ c₂ n l r v} (rb_l : IsRedBlack l c₁ n) (rb_r : IsRedBlack r c₂ n) :
-    is_bad_red_black (red_node l v r) n
-#align rbnode.is_bad_red_black Rbnode.IsBadRedBlack
+  bad_red {c₁ c₂ n l r v} (rb_l : Std.RBNode.IsRedBlack l c₁ n)
+    (rb_r : Std.RBNode.IsRedBlack r c₂ n) : is_bad_red_black (Std.RBNode.node l v r) n
+#align rbnode.is_bad_red_black Std.RBNode.IsBadRedBlack
 
-theorem balance1_rb {l r t : Rbnode α} {y v : α} {c_l c_r c_t n} :
-    IsRedBlack l c_l n →
-      IsRedBlack r c_r n → IsRedBlack t c_t n → ∃ c, IsRedBlack (balance1 l y r v t) c (succ n) :=
+theorem Std.RBNode.balance1_rb {l r t : Std.RBNode α} {y v : α} {c_l c_r c_t n} :
+    Std.RBNode.IsRedBlack l c_l n →
+      Std.RBNode.IsRedBlack r c_r n →
+        Std.RBNode.IsRedBlack t c_t n →
+          ∃ c, Std.RBNode.IsRedBlack (Std.RBNode.balance1 l y r v t) c (succ n) :=
   by
   intro h₁ h₂ _ <;> cases h₁ <;> cases h₂ <;>
     repeat'
       first
       | assumption
       | constructor
-#align rbnode.balance1_rb Rbnode.balance1_rb
+#align rbnode.balance1_rb Std.RBNode.balance1_rb
 
-theorem balance2_rb {l r t : Rbnode α} {y v : α} {c_l c_r c_t n} :
-    IsRedBlack l c_l n →
-      IsRedBlack r c_r n → IsRedBlack t c_t n → ∃ c, IsRedBlack (balance2 l y r v t) c (succ n) :=
+theorem Std.RBNode.balance2_rb {l r t : Std.RBNode α} {y v : α} {c_l c_r c_t n} :
+    Std.RBNode.IsRedBlack l c_l n →
+      Std.RBNode.IsRedBlack r c_r n →
+        Std.RBNode.IsRedBlack t c_t n →
+          ∃ c, Std.RBNode.IsRedBlack (Std.RBNode.balance2 l y r v t) c (succ n) :=
   by
   intro h₁ h₂ _ <;> cases h₁ <;> cases h₂ <;>
     repeat'
       first
       | assumption
       | constructor
-#align rbnode.balance2_rb Rbnode.balance2_rb
+#align rbnode.balance2_rb Std.RBNode.balance2_rb
 
-theorem balance1Node_rb {t s : Rbnode α} {y : α} {c n} :
-    IsBadRedBlack t n → IsRedBlack s c n → ∃ c, IsRedBlack (balance1Node t y s) c (succ n) := by
-  intro h _ <;> cases h <;> simp [balance1_node] <;> apply balance1_rb <;> assumption'
-#align rbnode.balance1_node_rb Rbnode.balance1Node_rb
+theorem Std.RBNode.balance1Node_rb {t s : Std.RBNode α} {y : α} {c n} :
+    Std.RBNode.IsBadRedBlack t n →
+      Std.RBNode.IsRedBlack s c n →
+        ∃ c, Std.RBNode.IsRedBlack (Std.RBNode.balance1Node t y s) c (succ n) :=
+  by intro h _ <;> cases h <;> simp [balance1_node] <;> apply balance1_rb <;> assumption'
+#align rbnode.balance1_node_rb Std.RBNode.balance1Node_rb
 
-theorem balance2Node_rb {t s : Rbnode α} {y : α} {c n} :
-    IsBadRedBlack t n → IsRedBlack s c n → ∃ c, IsRedBlack (balance2Node t y s) c (succ n) := by
-  intro h _ <;> cases h <;> simp [balance2_node] <;> apply balance2_rb <;> assumption'
-#align rbnode.balance2_node_rb Rbnode.balance2Node_rb
+theorem Std.RBNode.balance2Node_rb {t s : Std.RBNode α} {y : α} {c n} :
+    Std.RBNode.IsBadRedBlack t n →
+      Std.RBNode.IsRedBlack s c n →
+        ∃ c, Std.RBNode.IsRedBlack (Std.RBNode.balance2Node t y s) c (succ n) :=
+  by intro h _ <;> cases h <;> simp [balance2_node] <;> apply balance2_rb <;> assumption'
+#align rbnode.balance2_node_rb Std.RBNode.balance2Node_rb
 
-def InsRbResult : Rbnode α → Color → Nat → Prop
-  | t, red, n => IsBadRedBlack t n
-  | t, black, n => ∃ c, IsRedBlack t c n
-#align rbnode.ins_rb_result Rbnode.InsRbResult
+def Std.RBNode.InsRbResult : Std.RBNode α → RBColor → Nat → Prop
+  | t, red, n => Std.RBNode.IsBadRedBlack t n
+  | t, black, n => ∃ c, Std.RBNode.IsRedBlack t c n
+#align rbnode.ins_rb_result Std.RBNode.InsRbResult
 
 variable {lt : α → α → Prop} [DecidableRel lt]
 
-theorem of_getColor_eq_red {t : Rbnode α} {c n} : getColor t = red → IsRedBlack t c n → c = red :=
-  by intro h₁ h₂; cases h₂ <;> simp only [get_color] at h₁  <;> contradiction
-#align rbnode.of_get_color_eq_red Rbnode.of_getColor_eq_red
+theorem Std.RBNode.of_getColor_eq_red {t : Std.RBNode α} {c n} :
+    Std.RBNode.getColor t = red → Std.RBNode.IsRedBlack t c n → c = red := by intro h₁ h₂;
+  cases h₂ <;> simp only [get_color] at h₁  <;> contradiction
+#align rbnode.of_get_color_eq_red Std.RBNode.of_getColor_eq_red
 
-theorem of_getColor_ne_red {t : Rbnode α} {c n} : getColor t ≠ red → IsRedBlack t c n → c = black :=
-  by intro h₁ h₂; cases h₂ <;> simp only [get_color] at h₁  <;> contradiction
-#align rbnode.of_get_color_ne_red Rbnode.of_getColor_ne_red
+theorem Std.RBNode.of_getColor_ne_red {t : Std.RBNode α} {c n} :
+    Std.RBNode.getColor t ≠ red → Std.RBNode.IsRedBlack t c n → c = black := by intro h₁ h₂;
+  cases h₂ <;> simp only [get_color] at h₁  <;> contradiction
+#align rbnode.of_get_color_ne_red Std.RBNode.of_getColor_ne_red
 
 variable (lt)
 
-theorem ins_rb {t : Rbnode α} (x) : ∀ {c n} (h : IsRedBlack t c n), InsRbResult (ins lt t x) c n :=
+theorem Std.RBNode.ins_rb {t : Std.RBNode α} (x) :
+    ∀ {c n} (h : Std.RBNode.IsRedBlack t c n), Std.RBNode.InsRbResult (Std.RBNode.ins lt t x) c n :=
   by
   apply ins.induction lt t x <;> intros <;> cases h <;> simp [ins, *, ins_rb_result]
   · repeat' constructor
@@ -952,15 +1018,16 @@ theorem ins_rb {t : Rbnode α} (x) : ∀ {c n} (h : IsRedBlack t c n), InsRbResu
     cases of_get_color_ne_red hnr h_rb_r
     cases ih
     constructor; constructor <;> assumption
-#align rbnode.ins_rb Rbnode.ins_rb
+#align rbnode.ins_rb Std.RBNode.ins_rb
 
-def InsertRbResult : Rbnode α → Color → Nat → Prop
-  | t, red, n => IsRedBlack t black (succ n)
-  | t, black, n => ∃ c, IsRedBlack t c n
-#align rbnode.insert_rb_result Rbnode.InsertRbResult
+def Std.RBNode.InsertRbResult : Std.RBNode α → RBColor → Nat → Prop
+  | t, red, n => Std.RBNode.IsRedBlack t black (succ n)
+  | t, black, n => ∃ c, Std.RBNode.IsRedBlack t c n
+#align rbnode.insert_rb_result Std.RBNode.InsertRbResult
 
-theorem insert_rb {t : Rbnode α} (x) {c n} (h : IsRedBlack t c n) :
-    InsertRbResult (insert lt t x) c n := by
+theorem Std.RBNode.insert_rb {t : Std.RBNode α} (x) {c n} (h : Std.RBNode.IsRedBlack t c n) :
+    Std.RBNode.InsertRbResult (Std.RBNode.insert lt t x) c n :=
+  by
   simp [insert]
   have hi := ins_rb lt x h
   generalize he : ins lt t x = r
@@ -968,19 +1035,19 @@ theorem insert_rb {t : Rbnode α} (x) {c n} (h : IsRedBlack t c n) :
   cases h <;> simp [get_color, ins_rb_result, insert_rb_result, mk_insert_result] at *
   assumption'
   · cases hi; simp [mk_insert_result]; constructor <;> assumption
-#align rbnode.insert_rb Rbnode.insert_rb
+#align rbnode.insert_rb Std.RBNode.insert_rb
 
-theorem insert_isRedBlack {t : Rbnode α} {c n} (x) :
-    IsRedBlack t c n → ∃ c n, IsRedBlack (insert lt t x) c n :=
+theorem Std.RBNode.insert_isRedBlack {t : Std.RBNode α} {c n} (x) :
+    Std.RBNode.IsRedBlack t c n → ∃ c n, Std.RBNode.IsRedBlack (Std.RBNode.insert lt t x) c n :=
   by
   intro h
   have := insert_rb lt x h
   cases c <;> simp [insert_rb_result] at this 
   · constructor; constructor; assumption
   · cases this; constructor; constructor; assumption
-#align rbnode.insert_is_red_black Rbnode.insert_isRedBlack
+#align rbnode.insert_is_red_black Std.RBNode.insert_isRedBlack
 
 end IsRedBlack
 
-end Rbnode
+end Std.RBNode
 
