Mathbin/Data/Rbmap/Default.lean
@@ -31,7 +31,8 @@ private def rbmapLtDec {α : Type u} {β : Type v} {lt : α → α → Prop} [h 
 attribute [local instance] rbmap_lt_is_swo rbmap_lt_dec
 
 -- Helper lemmas for reusing rbtree results.
-private theorem to_rbtree_mem {k : α} {m : Rbmap α β lt} : k ∈ m → ∃ v : β, Rbtree.Mem (k, v) m :=
+private theorem to_rbtree_mem {k : α} {m : Rbmap α β lt} :
+    k ∈ m → ∃ v : β, Std.RBSet.Mem (k, v) m :=
   by
   cases' m with n p <;> cases n <;> intro h
   · exact False.elim h
@@ -49,24 +50,24 @@ private theorem eqv_entries [IsIrrefl α lt] (k : α) (v₁ v₂ : β) : (k, v�
   And.intro (irrefl_of lt k) (irrefl_of lt k)
 
 private theorem to_rbmap_mem [IsStrictWeakOrder α lt] {k : α} {v : β} {m : Rbmap α β lt} :
-    Rbtree.Mem (k, v) m → k ∈ m :=
+    Std.RBSet.Mem (k, v) m → k ∈ m :=
   by
   cases' m with n p <;> cases n <;> intro h
   · exact False.elim h
   · simp [Membership.Mem, Rbmap.Mem]
     exact
-      @Rbtree.mem_of_mem_of_eqv _ _ _ ⟨Rbnode.red_node n_lchild n_val n_rchild, p⟩ _ _ h
+      @Std.RBSet.mem_of_mem_of_eqv _ _ _ ⟨Std.RBNode.node n_lchild n_val n_rchild, p⟩ _ _ h
         (eqv_entries _ _ _)
   · simp [Membership.Mem, Rbmap.Mem]
     exact
-      @Rbtree.mem_of_mem_of_eqv _ _ _ ⟨Rbnode.black_node n_lchild n_val n_rchild, p⟩ _ _ h
+      @Std.RBSet.mem_of_mem_of_eqv _ _ _ ⟨rbnode.black_node n_lchild n_val n_rchild, p⟩ _ _ h
         (eqv_entries _ _ _)
 
 private theorem to_rbtree_mem' [IsStrictWeakOrder α lt] {k : α} {m : Rbmap α β lt} (v : β) :
-    k ∈ m → Rbtree.Mem (k, v) m := by
+    k ∈ m → Std.RBSet.Mem (k, v) m := by
   intro h
   cases' to_rbtree_mem h with v' hm
-  apply Rbtree.mem_of_mem_of_eqv hm
+  apply Std.RBSet.mem_of_mem_of_eqv hm
   apply eqv_entries
 
 theorem eq_some_of_toValue_eq_some {e : Option (α × β)} {v : β} :
@@ -82,19 +83,20 @@ theorem eq_none_of_toValue_eq_none {e : Option (α × β)} : toValue e = none �
 
 -- Lemmas
 theorem not_mem_mkRbmap : ∀ k : α, k ∉ mkRbmap α β lt := by
-  simp [Membership.Mem, mkRbmap, mkRbtree, Rbmap.Mem]
+  simp [Membership.Mem, mkRbmap, Std.mkRBSet, Rbmap.Mem]
 #align rbmap.not_mem_mk_rbmap Rbmap.not_mem_mkRbmap
 
 theorem not_mem_of_empty {m : Rbmap α β lt} (k : α) : m.Empty = true → k ∉ m := by
   cases' m with n p <;> cases n <;>
-    simp [Membership.Mem, mkRbmap, mkRbtree, Rbmap.Mem, Rbmap.empty, Rbtree.empty, false_imp_iff]
+    simp [Membership.Mem, mkRbmap, Std.mkRBSet, Rbmap.Mem, Rbmap.empty, Std.RBSet.empty,
+      false_imp_iff]
 #align rbmap.not_mem_of_empty Rbmap.not_mem_of_empty
 
 theorem mem_of_mem_of_eqv [IsStrictWeakOrder α lt] {m : Rbmap α β lt} {k₁ k₂ : α} :
     k₁ ∈ m → k₁ ≈[lt]k₂ → k₂ ∈ m := by
   intro h₁ h₂
   have h₁ := to_rbtree_mem h₁; cases' h₁ with v h₁
-  exact to_rbmap_mem (Rbtree.mem_of_mem_of_eqv h₁ (eqv_entries_of_eqv_keys v v h₂))
+  exact to_rbmap_mem (Std.RBSet.mem_of_mem_of_eqv h₁ (eqv_entries_of_eqv_keys v v h₂))
 #align rbmap.mem_of_mem_of_eqv Rbmap.mem_of_mem_of_eqv
 
 section Decidable
@@ -105,7 +107,7 @@ theorem not_mem_of_findEntry_none [IsStrictWeakOrder α lt] {k : α} {m : Rbmap 
     m.findEntry k = none → k ∉ m := by
   cases' m with t p; cases t <;> simp [find_entry]
   · intros; simp [Membership.Mem, Rbmap.Mem]
-  all_goals intro h; exact Rbtree.not_mem_of_find_none h
+  all_goals intro h; exact Std.RBSet.not_mem_of_find?_none h
 #align rbmap.not_mem_of_find_entry_none Rbmap.not_mem_of_findEntry_none
 
 theorem not_mem_of_find_none [IsStrictWeakOrder α lt] {k : α} {m : Rbmap α β lt} :
@@ -118,7 +120,7 @@ theorem not_mem_of_find_none [IsStrictWeakOrder α lt] {k : α} {m : Rbmap α β
 theorem mem_of_findEntry_some [IsStrictWeakOrder α lt] {k₁ : α} {e : α × β} {m : Rbmap α β lt} :
     m.findEntry k₁ = some e → k₁ ∈ m := by
   cases' m with t p; cases t <;> simp [find_entry, false_imp_iff]
-  all_goals intro h; exact Rbtree.mem_of_find_some h
+  all_goals intro h; exact Std.RBSet.mem_of_find?_some h
 #align rbmap.mem_of_find_entry_some Rbmap.mem_of_findEntry_some
 
 theorem mem_of_find_some [IsStrictWeakOrder α lt] {k : α} {v : β} {m : Rbmap α β lt} :
@@ -133,7 +135,7 @@ theorem findEntry_eq_findEntry_of_eqv [IsStrictWeakOrder α lt] {m : Rbmap α β
     k₁ ≈[lt]k₂ → m.findEntry k₁ = m.findEntry k₂ :=
   by
   intro h; cases' m with t p; cases t <;> simp [find_entry]
-  all_goals apply Rbtree.find_eq_find_of_eqv; apply eqv_entries_of_eqv_keys; assumption
+  all_goals apply Std.RBSet.find?_eq_find?_of_eqv; apply eqv_entries_of_eqv_keys; assumption
 #align rbmap.find_entry_eq_find_entry_of_eqv Rbmap.findEntry_eq_findEntry_of_eqv
 
 theorem find_eq_find_of_eqv [IsStrictWeakOrder α lt] {k₁ k₂ : α} (m : Rbmap α β lt) :
@@ -147,32 +149,32 @@ theorem findEntry_correct [IsStrictWeakOrder α lt] (k : α) (m : Rbmap α β lt
   apply Iff.intro <;> cases' m with t p
   · intro h
     have h := to_rbtree_mem h; cases' h with v h₁
-    have hex := Iff.mp (Rbtree.find_correct _ _) h₁; cases' hex with e h₂
+    have hex := Iff.mp (Std.RBSet.find?_correct _ _) h₁; cases' hex with e h₂
     exists e; cases t <;> simp [find_entry] at h₂ ⊢
-    · simp [Rbtree.find, Rbnode.find] at h₂ ; cases h₂
+    · simp [Std.RBSet.find?, Std.RBNode.find?] at h₂ ; cases h₂
     · cases' h₂ with h₂₁ h₂₂; constructor
       · have :=
-          Rbtree.find_eq_find_of_eqv ⟨Rbnode.red_node t_lchild t_val t_rchild, p⟩
+          Std.RBSet.find?_eq_find?_of_eqv ⟨Std.RBNode.node t_lchild t_val t_rchild, p⟩
             (eqv_entries k v t_val.2)
         rw [← this]; exact h₂₁
       · cases e; apply eqv_keys_of_eqv_entries h₂₂
     · cases' h₂ with h₂₁ h₂₂; constructor
       · have :=
-          Rbtree.find_eq_find_of_eqv ⟨Rbnode.black_node t_lchild t_val t_rchild, p⟩
+          Std.RBSet.find?_eq_find?_of_eqv ⟨rbnode.black_node t_lchild t_val t_rchild, p⟩
             (eqv_entries k v t_val.2)
         rw [← this]; exact h₂₁
       · cases e; apply eqv_keys_of_eqv_entries h₂₂
   · intro h; cases' h with e h
     cases' h with h₁ h₂; cases t <;> simp [find_entry] at h₁ 
     · contradiction
-    all_goals exact to_rbmap_mem (Rbtree.mem_of_find_some h₁)
+    all_goals exact to_rbmap_mem (Std.RBSet.mem_of_find?_some h₁)
 #align rbmap.find_entry_correct Rbmap.findEntry_correct
 
 theorem eqv_of_findEntry_some [IsStrictWeakOrder α lt] {k₁ k₂ : α} {v : β} {m : Rbmap α β lt} :
     m.findEntry k₁ = some (k₂, v) → k₁ ≈[lt]k₂ :=
   by
   cases' m with t p; cases t <;> simp [find_entry, false_imp_iff]
-  all_goals intro h; exact eqv_keys_of_eqv_entries (Rbtree.eqv_of_find_some h)
+  all_goals intro h; exact eqv_keys_of_eqv_entries (Std.RBSet.eqv_of_find?_some h)
 #align rbmap.eqv_of_find_entry_some Rbmap.eqv_of_findEntry_some
 
 theorem eq_of_findEntry_some [IsStrictTotalOrder α lt] {k₁ k₂ : α} {v : β} {m : Rbmap α β lt} :
@@ -214,11 +216,11 @@ theorem constains_correct [IsStrictWeakOrder α lt] (k : α) (m : Rbmap α β lt
 
 theorem mem_insert_of_incomp [IsStrictWeakOrder α lt] {k₁ k₂ : α} (m : Rbmap α β lt) (v : β) :
     ¬lt k₁ k₂ ∧ ¬lt k₂ k₁ → k₁ ∈ m.insert k₂ v := fun h =>
-  to_rbmap_mem (Rbtree.mem_insert_of_incomp m (eqv_entries_of_eqv_keys v v h))
+  to_rbmap_mem (Std.RBSet.mem_insert_of_incomp m (eqv_entries_of_eqv_keys v v h))
 #align rbmap.mem_insert_of_incomp Rbmap.mem_insert_of_incomp
 
 theorem mem_insert [IsStrictWeakOrder α lt] (k : α) (m : Rbmap α β lt) (v : β) : k ∈ m.insert k v :=
-  to_rbmap_mem (Rbtree.mem_insert (k, v) m)
+  to_rbmap_mem (Std.RBSet.mem_insert (k, v) m)
 #align rbmap.mem_insert Rbmap.mem_insert
 
 theorem mem_insert_of_equiv [IsStrictWeakOrder α lt] {k₁ k₂ : α} (m : Rbmap α β lt) (v : β) :
@@ -228,12 +230,12 @@ theorem mem_insert_of_equiv [IsStrictWeakOrder α lt] {k₁ k₂ : α} (m : Rbma
 
 theorem mem_insert_of_mem [IsStrictWeakOrder α lt] {k₁ : α} {m : Rbmap α β lt} (k₂ : α) (v : β) :
     k₁ ∈ m → k₁ ∈ m.insert k₂ v := fun h =>
-  to_rbmap_mem (Rbtree.mem_insert_of_mem (k₂, v) (to_rbtree_mem' v h))
+  to_rbmap_mem (Std.RBSet.mem_insert_of_mem (k₂, v) (to_rbtree_mem' v h))
 #align rbmap.mem_insert_of_mem Rbmap.mem_insert_of_mem
 
 theorem equiv_or_mem_of_mem_insert [IsStrictWeakOrder α lt] {k₁ k₂ : α} {v : β} {m : Rbmap α β lt} :
     k₁ ∈ m.insert k₂ v → k₁ ≈[lt]k₂ ∨ k₁ ∈ m := fun h =>
-  Or.elim (Rbtree.equiv_or_mem_of_mem_insert (to_rbtree_mem' v h))
+  Or.elim (Std.RBSet.equiv_or_mem_of_mem_insert (to_rbtree_mem' v h))
     (fun h => Or.inl (eqv_keys_of_eqv_entries h)) fun h => Or.inr (to_rbmap_mem h)
 #align rbmap.equiv_or_mem_of_mem_insert Rbmap.equiv_or_mem_of_mem_insert
 
@@ -256,7 +258,7 @@ theorem findEntry_insert_of_eqv [IsStrictWeakOrder α lt] (m : Rbmap α β lt) {
   cases' m' with t p; cases t
   · have := mem_insert k₁ m v; rw [h₁] at this ; apply absurd this; apply not_mem_mk_rbmap
   all_goals
-    simp [find_entry]; rw [← h₁, insert]; apply Rbtree.find_insert_of_eqv
+    simp [find_entry]; rw [← h₁, insert]; apply Std.RBSet.find?_insert_of_eqv
     apply eqv_entries_of_eqv_keys _ _ h
 #align rbmap.find_entry_insert_of_eqv Rbmap.findEntry_insert_of_eqv
 
@@ -294,14 +296,14 @@ theorem findEntry_insert_of_disj [IsStrictWeakOrder α lt] {k₁ k₂ : α} (m :
     conv =>
       lhs
       simp [find_entry]
-    rw [← h₂, insert, Rbtree.find_insert_of_disj _ h', h₁]
+    rw [← h₂, insert, Std.RBSet.find?_insert_of_disj _ h', h₁]
     rfl
   any_goals
     simp [insert] at h₂ 
-    exact absurd h₂ (Rbtree.insert_ne_mkRbtree m (k₁, v))
+    exact absurd h₂ (Std.RBSet.insert_ne_mkRBSet m (k₁, v))
   any_goals
-    rw [h₂, h₁]; simp [find_entry]; rw [← h₂, ← h₁, insert, Rbtree.find_insert_of_disj _ h']
-    apply Rbtree.find_eq_find_of_eqv; apply eqv_entries
+    rw [h₂, h₁]; simp [find_entry]; rw [← h₂, ← h₁, insert, Std.RBSet.find?_insert_of_disj _ h']
+    apply Std.RBSet.find?_eq_find?_of_eqv; apply eqv_entries
 #align rbmap.find_entry_insert_of_disj Rbmap.findEntry_insert_of_disj
 
 theorem findEntry_insert_of_not_eqv [IsStrictWeakOrder α lt] {k₁ k₂ : α} (m : Rbmap α β lt)
@@ -341,30 +343,30 @@ theorem find_insert_of_ne [IsStrictTotalOrder α lt] {k₁ k₂ : α} (m : Rbmap
 end Decidable
 
 theorem mem_of_min_eq [IsStrictTotalOrder α lt] {k : α} {v : β} {m : Rbmap α β lt} :
-    m.min = some (k, v) → k ∈ m := fun h => to_rbmap_mem (Rbtree.mem_of_min_eq h)
+    m.min = some (k, v) → k ∈ m := fun h => to_rbmap_mem (Std.RBSet.mem_of_min_eq h)
 #align rbmap.mem_of_min_eq Rbmap.mem_of_min_eq
 
 theorem mem_of_max_eq [IsStrictTotalOrder α lt] {k : α} {v : β} {m : Rbmap α β lt} :
-    m.max = some (k, v) → k ∈ m := fun h => to_rbmap_mem (Rbtree.mem_of_max_eq h)
+    m.max = some (k, v) → k ∈ m := fun h => to_rbmap_mem (Std.RBSet.mem_of_max_eq h)
 #align rbmap.mem_of_max_eq Rbmap.mem_of_max_eq
 
 theorem eq_leaf_of_min_eq_none {m : Rbmap α β lt} : m.min = none → m = mkRbmap α β lt :=
-  Rbtree.eq_leaf_of_min_eq_none
+  Std.RBSet.eq_leaf_of_min_eq_none
 #align rbmap.eq_leaf_of_min_eq_none Rbmap.eq_leaf_of_min_eq_none
 
 theorem eq_leaf_of_max_eq_none {m : Rbmap α β lt} : m.max = none → m = mkRbmap α β lt :=
-  Rbtree.eq_leaf_of_max_eq_none
+  Std.RBSet.eq_leaf_of_max_eq_none
 #align rbmap.eq_leaf_of_max_eq_none Rbmap.eq_leaf_of_max_eq_none
 
 theorem min_is_minimal [IsStrictWeakOrder α lt] {k : α} {v : β} {m : Rbmap α β lt} :
     m.min = some (k, v) → ∀ {k'}, k' ∈ m → k ≈[lt]k' ∨ lt k k' := fun h k' hm =>
-  Or.elim (Rbtree.min_is_minimal h (to_rbtree_mem' v hm))
+  Or.elim (Std.RBSet.min_is_minimal h (to_rbtree_mem' v hm))
     (fun h => Or.inl (eqv_keys_of_eqv_entries h)) fun h => Or.inr h
 #align rbmap.min_is_minimal Rbmap.min_is_minimal
 
 theorem max_is_maximal [IsStrictWeakOrder α lt] {k : α} {v : β} {m : Rbmap α β lt} :
     m.max = some (k, v) → ∀ {k'}, k' ∈ m → k ≈[lt]k' ∨ lt k' k := fun h k' hm =>
-  Or.elim (Rbtree.max_is_maximal h (to_rbtree_mem' v hm))
+  Or.elim (Std.RBSet.max_is_maximal h (to_rbtree_mem' v hm))
     (fun h => Or.inl (eqv_keys_of_eqv_entries h)) fun h => Or.inr h
 #align rbmap.max_is_maximal Rbmap.max_is_maximal
 
