Mathbin/Data/Rbtree/Main.lean
@@ -15,157 +15,166 @@ import Mathbin.Order.RelClasses
 
 universe u
 
-namespace Rbnode
+namespace Std.RBNode
 
 variable {α : Type u} {lt : α → α → Prop}
 
-theorem isSearchable_of_wellFormed {t : Rbnode α} [IsStrictWeakOrder α lt] :
-    t.WellFormed lt → IsSearchable lt t none none :=
+theorem Std.RBNode.isSearchableOfWellFormed {t : Std.RBNode α} [IsStrictWeakOrder α lt] :
+    t.WF lt → Std.RBNode.IsSearchable lt t none none :=
   by
   intro h; induction h
   · constructor; simp [lift]
   · subst h_n'; apply is_searchable_insert; assumption
-#align rbnode.is_searchable_of_well_formed Rbnode.isSearchable_of_wellFormed
+#align rbnode.is_searchable_of_well_formed Std.RBNode.isSearchableOfWellFormed
 
 open Color
 
-theorem isRedBlack_of_wellFormed {t : Rbnode α} : t.WellFormed lt → ∃ c n, IsRedBlack t c n :=
+theorem Std.RBNode.isRedBlack_of_wF {t : Std.RBNode α} :
+    t.WF lt → ∃ c n, Std.RBNode.IsRedBlack t c n :=
   by
   intro h; induction h
   · exists black; exists 0; constructor
   · cases' h_ih with c ih; cases' ih with n ih; subst h_n'; apply insert_is_red_black; assumption
-#align rbnode.is_red_black_of_well_formed Rbnode.isRedBlack_of_wellFormed
+#align rbnode.is_red_black_of_well_formed Std.RBNode.isRedBlack_of_wF
 
-end Rbnode
+end Std.RBNode
 
-namespace Rbtree
+namespace Std.RBSet
 
 variable {α : Type u} {lt : α → α → Prop}
 
-theorem balanced (t : Rbtree α lt) : t.depth max ≤ 2 * t.depth min + 1 :=
+theorem Std.RBSet.balanced (t : Std.RBSet α lt) : t.depth max ≤ 2 * t.depth min + 1 :=
   by
   cases' t with n p; simp only [depth]
-  have := Rbnode.isRedBlack_of_wellFormed p
+  have := Std.RBNode.isRedBlack_of_wF p
   cases' this with _ this; cases' this with _ this
-  apply Rbnode.balanced; assumption
-#align rbtree.balanced Rbtree.balanced
+  apply Std.RBNode.balanced; assumption
+#align rbtree.balanced Std.RBSet.balanced
 
-theorem not_mem_mkRbtree : ∀ a : α, a ∉ mkRbtree α lt := by
-  simp [Membership.Mem, Rbtree.Mem, Rbnode.Mem, mkRbtree]
-#align rbtree.not_mem_mk_rbtree Rbtree.not_mem_mkRbtree
+theorem Std.RBSet.not_mem_mkRBSet : ∀ a : α, a ∉ Std.mkRBSet α lt := by
+  simp [Membership.Mem, Std.RBSet.Mem, Std.RBNode.Mem, Std.mkRBSet]
+#align rbtree.not_mem_mk_rbtree Std.RBSet.not_mem_mkRBSet
 
-theorem not_mem_of_empty {t : Rbtree α lt} (a : α) : t.Empty = true → a ∉ t := by
+theorem Std.RBSet.not_mem_of_empty {t : Std.RBSet α lt} (a : α) : t.Empty = true → a ∉ t := by
   cases' t with n p <;> cases n <;>
-    simp [Empty, Membership.Mem, Rbtree.Mem, Rbnode.Mem, false_imp_iff]
-#align rbtree.not_mem_of_empty Rbtree.not_mem_of_empty
+    simp [Empty, Membership.Mem, Std.RBSet.Mem, Std.RBNode.Mem, false_imp_iff]
+#align rbtree.not_mem_of_empty Std.RBSet.not_mem_of_empty
 
-theorem mem_of_mem_of_eqv [IsStrictWeakOrder α lt] {t : Rbtree α lt} {a b : α} :
+theorem Std.RBSet.mem_of_mem_of_eqv [IsStrictWeakOrder α lt] {t : Std.RBSet α lt} {a b : α} :
     a ∈ t → a ≈[lt]b → b ∈ t :=
   by
-  cases' t with n p <;> simp [Membership.Mem, Rbtree.Mem] <;> clear p <;> induction n <;>
-        simp only [Rbnode.Mem, StrictWeakOrder.Equiv, false_imp_iff] <;>
+  cases' t with n p <;> simp [Membership.Mem, Std.RBSet.Mem] <;> clear p <;> induction n <;>
+        simp only [Std.RBNode.Mem, StrictWeakOrder.Equiv, false_imp_iff] <;>
       intro h₁ h₂ <;>
     cases_type* or.1
   iterate 2 
-    · have : Rbnode.Mem lt b n_lchild := n_ih_lchild h₁ h₂; simp [this]
+    · have : Std.RBNode.Mem lt b n_lchild := n_ih_lchild h₁ h₂; simp [this]
     · simp [incomp_trans_of lt h₂.swap h₁]
-    · have : Rbnode.Mem lt b n_rchild := n_ih_rchild h₁ h₂; simp [this]
-#align rbtree.mem_of_mem_of_eqv Rbtree.mem_of_mem_of_eqv
+    · have : Std.RBNode.Mem lt b n_rchild := n_ih_rchild h₁ h₂; simp [this]
+#align rbtree.mem_of_mem_of_eqv Std.RBSet.mem_of_mem_of_eqv
 
 section Dec
 
 variable [DecidableRel lt]
 
-theorem insert_ne_mkRbtree (t : Rbtree α lt) (a : α) : t.insert a ≠ mkRbtree α lt :=
+theorem Std.RBSet.insert_ne_mkRBSet (t : Std.RBSet α lt) (a : α) : t.insert a ≠ Std.mkRBSet α lt :=
   by
   cases' t with n p
-  simpa [insert, mkRbtree] using Rbnode.insert_ne_leaf lt n a
-#align rbtree.insert_ne_mk_rbtree Rbtree.insert_ne_mkRbtree
+  simpa [insert, Std.mkRBSet] using Std.RBNode.insert_ne_nil lt n a
+#align rbtree.insert_ne_mk_rbtree Std.RBSet.insert_ne_mkRBSet
 
-theorem find_correct [IsStrictWeakOrder α lt] (a : α) (t : Rbtree α lt) :
-    a ∈ t ↔ ∃ b, t.find a = some b ∧ a ≈[lt]b := by cases t; apply Rbnode.find_correct;
-  apply Rbnode.isSearchable_of_wellFormed; assumption
-#align rbtree.find_correct Rbtree.find_correct
+theorem Std.RBSet.find?_correct [IsStrictWeakOrder α lt] (a : α) (t : Std.RBSet α lt) :
+    a ∈ t ↔ ∃ b, t.find a = some b ∧ a ≈[lt]b := by cases t; apply Std.RBNode.find?_correct;
+  apply Std.RBNode.isSearchableOfWellFormed; assumption
+#align rbtree.find_correct Std.RBSet.find?_correct
 
-theorem find_correct_of_total [IsStrictTotalOrder α lt] (a : α) (t : Rbtree α lt) :
+theorem Std.RBSet.find?_correct_of_total [IsStrictTotalOrder α lt] (a : α) (t : Std.RBSet α lt) :
     a ∈ t ↔ t.find a = some a :=
   Iff.intro
     (fun h =>
-      match Iff.mp (find_correct a t) h with
+      match Iff.mp (Std.RBSet.find?_correct a t) h with
       | ⟨b, HEq, heqv⟩ => by simp [HEq, (eq_of_eqv_lt heqv).symm])
-    fun h => Iff.mpr (find_correct a t) ⟨a, ⟨h, refl a⟩⟩
-#align rbtree.find_correct_of_total Rbtree.find_correct_of_total
+    fun h => Iff.mpr (Std.RBSet.find?_correct a t) ⟨a, ⟨h, refl a⟩⟩
+#align rbtree.find_correct_of_total Std.RBSet.find?_correct_of_total
 
-theorem find_correct_exact [IsStrictTotalOrder α lt] (a : α) (t : Rbtree α lt) :
-    MemExact a t ↔ t.find a = some a := by cases t; apply Rbnode.find_correct_exact;
-  apply Rbnode.isSearchable_of_wellFormed; assumption
-#align rbtree.find_correct_exact Rbtree.find_correct_exact
+theorem Std.RBSet.find?_correct_exact [IsStrictTotalOrder α lt] (a : α) (t : Std.RBSet α lt) :
+    Std.RBSet.MemExact a t ↔ t.find a = some a := by cases t; apply Std.RBNode.find?_correct_exact;
+  apply Std.RBNode.isSearchableOfWellFormed; assumption
+#align rbtree.find_correct_exact Std.RBSet.find?_correct_exact
 
-theorem find_insert_of_eqv [IsStrictWeakOrder α lt] (t : Rbtree α lt) {x y} :
+theorem Std.RBSet.find?_insert_of_eqv [IsStrictWeakOrder α lt] (t : Std.RBSet α lt) {x y} :
     x ≈[lt]y → (t.insert x).find y = some x :=
   by
-  cases t; intro h; apply Rbnode.find_insert_of_eqv lt h; apply Rbnode.isSearchable_of_wellFormed
+  cases t; intro h; apply Std.RBNode.find?_insert_of_eqv lt h;
+  apply Std.RBNode.isSearchableOfWellFormed
   assumption
-#align rbtree.find_insert_of_eqv Rbtree.find_insert_of_eqv
+#align rbtree.find_insert_of_eqv Std.RBSet.find?_insert_of_eqv
 
-theorem find_insert [IsStrictWeakOrder α lt] (t : Rbtree α lt) (x) : (t.insert x).find x = some x :=
-  find_insert_of_eqv t (refl x)
-#align rbtree.find_insert Rbtree.find_insert
+#print Std.RBSet.find?_insert /-
+theorem Std.RBSet.find?_insert [IsStrictWeakOrder α lt] (t : Std.RBSet α lt) (x) :
+    (t.insert x).find x = some x :=
+  Std.RBSet.find?_insert_of_eqv t (refl x)
+#align rbtree.find_insert Std.RBSet.find?_insert
+-/
 
-theorem find_insert_of_disj [IsStrictWeakOrder α lt] {x y : α} (t : Rbtree α lt) :
+theorem Std.RBSet.find?_insert_of_disj [IsStrictWeakOrder α lt] {x y : α} (t : Std.RBSet α lt) :
     lt x y ∨ lt y x → (t.insert x).find y = t.find y :=
   by
-  cases t; intro h; apply Rbnode.find_insert_of_disj lt h
-  apply Rbnode.isSearchable_of_wellFormed
+  cases t; intro h; apply Std.RBNode.find?_insert_of_disj lt h
+  apply Std.RBNode.isSearchableOfWellFormed
   assumption
-#align rbtree.find_insert_of_disj Rbtree.find_insert_of_disj
+#align rbtree.find_insert_of_disj Std.RBSet.find?_insert_of_disj
 
-theorem find_insert_of_not_eqv [IsStrictWeakOrder α lt] {x y : α} (t : Rbtree α lt) :
+theorem Std.RBSet.find?_insert_of_not_eqv [IsStrictWeakOrder α lt] {x y : α} (t : Std.RBSet α lt) :
     ¬x ≈[lt]y → (t.insert x).find y = t.find y :=
   by
-  cases t; intro h; apply Rbnode.find_insert_of_not_eqv lt h
-  apply Rbnode.isSearchable_of_wellFormed; assumption
-#align rbtree.find_insert_of_not_eqv Rbtree.find_insert_of_not_eqv
+  cases t; intro h; apply Std.RBNode.find?_insert_of_not_eqv lt h
+  apply Std.RBNode.isSearchableOfWellFormed; assumption
+#align rbtree.find_insert_of_not_eqv Std.RBSet.find?_insert_of_not_eqv
 
-theorem find_insert_of_ne [IsStrictTotalOrder α lt] {x y : α} (t : Rbtree α lt) :
+#print Std.RBSet.find?_insert_of_ne /-
+theorem Std.RBSet.find?_insert_of_ne [IsStrictTotalOrder α lt] {x y : α} (t : Std.RBSet α lt) :
     x ≠ y → (t.insert x).find y = t.find y :=
   by
   cases t; intro h
   have : ¬x ≈[lt]y := fun h' => h (eq_of_eqv_lt h')
-  apply Rbnode.find_insert_of_not_eqv lt this
-  apply Rbnode.isSearchable_of_wellFormed; assumption
-#align rbtree.find_insert_of_ne Rbtree.find_insert_of_ne
+  apply Std.RBNode.find?_insert_of_not_eqv lt this
+  apply Std.RBNode.isSearchableOfWellFormed; assumption
+#align rbtree.find_insert_of_ne Std.RBSet.find?_insert_of_ne
+-/
 
-theorem not_mem_of_find_none [IsStrictWeakOrder α lt] {a : α} {t : Rbtree α lt} :
+theorem Std.RBSet.not_mem_of_find?_none [IsStrictWeakOrder α lt] {a : α} {t : Std.RBSet α lt} :
     t.find a = none → a ∉ t := fun h =>
-  Iff.mpr (not_congr (find_correct a t)) <| by
+  Iff.mpr (not_congr (Std.RBSet.find?_correct a t)) <|
+    by
     intro h
     cases' h with _ h; cases' h with h₁ h₂
     rw [h] at h₁ ; contradiction
-#align rbtree.not_mem_of_find_none Rbtree.not_mem_of_find_none
+#align rbtree.not_mem_of_find_none Std.RBSet.not_mem_of_find?_none
 
-theorem eqv_of_find_some [IsStrictWeakOrder α lt] {a b : α} {t : Rbtree α lt} :
-    t.find a = some b → a ≈[lt]b := by cases t; apply Rbnode.eqv_of_find_some;
-  apply Rbnode.isSearchable_of_wellFormed; assumption
-#align rbtree.eqv_of_find_some Rbtree.eqv_of_find_some
+theorem Std.RBSet.eqv_of_find?_some [IsStrictWeakOrder α lt] {a b : α} {t : Std.RBSet α lt} :
+    t.find a = some b → a ≈[lt]b := by cases t; apply Std.RBNode.eqv_of_find?_some;
+  apply Std.RBNode.isSearchableOfWellFormed; assumption
+#align rbtree.eqv_of_find_some Std.RBSet.eqv_of_find?_some
 
-theorem eq_of_find_some [IsStrictTotalOrder α lt] {a b : α} {t : Rbtree α lt} :
+theorem Std.RBSet.eq_of_find?_some [IsStrictTotalOrder α lt] {a b : α} {t : Std.RBSet α lt} :
     t.find a = some b → a = b := fun h =>
   suffices a ≈[lt]b from eq_of_eqv_lt this
-  eqv_of_find_some h
-#align rbtree.eq_of_find_some Rbtree.eq_of_find_some
+  Std.RBSet.eqv_of_find?_some h
+#align rbtree.eq_of_find_some Std.RBSet.eq_of_find?_some
 
-theorem mem_of_find_some [IsStrictWeakOrder α lt] {a b : α} {t : Rbtree α lt} :
-    t.find a = some b → a ∈ t := fun h => Iff.mpr (find_correct a t) ⟨b, ⟨h, eqv_of_find_some h⟩⟩
-#align rbtree.mem_of_find_some Rbtree.mem_of_find_some
+theorem Std.RBSet.mem_of_find?_some [IsStrictWeakOrder α lt] {a b : α} {t : Std.RBSet α lt} :
+    t.find a = some b → a ∈ t := fun h =>
+  Iff.mpr (Std.RBSet.find?_correct a t) ⟨b, ⟨h, Std.RBSet.eqv_of_find?_some h⟩⟩
+#align rbtree.mem_of_find_some Std.RBSet.mem_of_find?_some
 
-theorem find_eq_find_of_eqv [IsStrictWeakOrder α lt] {a b : α} (t : Rbtree α lt) :
+theorem Std.RBSet.find?_eq_find?_of_eqv [IsStrictWeakOrder α lt] {a b : α} (t : Std.RBSet α lt) :
     a ≈[lt]b → t.find a = t.find b := by
-  cases t; apply Rbnode.find_eq_find_of_eqv
-  apply Rbnode.isSearchable_of_wellFormed; assumption
-#align rbtree.find_eq_find_of_eqv Rbtree.find_eq_find_of_eqv
+  cases t; apply Std.RBNode.find?_eq_find?_of_eqv
+  apply Std.RBNode.isSearchableOfWellFormed; assumption
+#align rbtree.find_eq_find_of_eqv Std.RBSet.find?_eq_find?_of_eqv
 
-theorem contains_correct [IsStrictWeakOrder α lt] (a : α) (t : Rbtree α lt) :
+theorem Std.RBSet.contains_correct [IsStrictWeakOrder α lt] (a : α) (t : Std.RBSet α lt) :
     a ∈ t ↔ t.contains a = true := by
   have h := find_correct a t
   simp [h, contains]; apply Iff.intro
@@ -173,70 +182,76 @@ theorem contains_correct [IsStrictWeakOrder α lt] (a : α) (t : Rbtree α lt) :
   · intro h'
     cases' heq : find t a with v; simp [HEq, Option.isSome] at h' ; contradiction
     exists v; simp; apply eqv_of_find_some HEq
-#align rbtree.contains_correct Rbtree.contains_correct
+#align rbtree.contains_correct Std.RBSet.contains_correct
 
-theorem mem_insert_of_incomp {a b : α} (t : Rbtree α lt) : ¬lt a b ∧ ¬lt b a → a ∈ t.insert b := by
-  cases t; apply Rbnode.mem_insert_of_incomp
-#align rbtree.mem_insert_of_incomp Rbtree.mem_insert_of_incomp
+theorem Std.RBSet.mem_insert_of_incomp {a b : α} (t : Std.RBSet α lt) :
+    ¬lt a b ∧ ¬lt b a → a ∈ t.insert b := by cases t; apply Std.RBNode.mem_insert_of_incomp
+#align rbtree.mem_insert_of_incomp Std.RBSet.mem_insert_of_incomp
 
-theorem mem_insert [IsIrrefl α lt] : ∀ (a : α) (t : Rbtree α lt), a ∈ t.insert a := by intros;
-  apply mem_insert_of_incomp; constructor <;> apply irrefl_of lt
-#align rbtree.mem_insert Rbtree.mem_insert
+#print Std.RBSet.mem_insert /-
+theorem Std.RBSet.mem_insert [IsIrrefl α lt] : ∀ (a : α) (t : Std.RBSet α lt), a ∈ t.insert a := by
+  intros; apply mem_insert_of_incomp; constructor <;> apply irrefl_of lt
+#align rbtree.mem_insert Std.RBSet.mem_insert
+-/
 
-theorem mem_insert_of_equiv {a b : α} (t : Rbtree α lt) : a ≈[lt]b → a ∈ t.insert b := by cases t;
-  apply Rbnode.mem_insert_of_incomp
-#align rbtree.mem_insert_of_equiv Rbtree.mem_insert_of_equiv
+theorem Std.RBSet.mem_insert_of_equiv {a b : α} (t : Std.RBSet α lt) : a ≈[lt]b → a ∈ t.insert b :=
+  by cases t; apply Std.RBNode.mem_insert_of_incomp
+#align rbtree.mem_insert_of_equiv Std.RBSet.mem_insert_of_equiv
 
-theorem mem_insert_of_mem [IsStrictWeakOrder α lt] {a : α} {t : Rbtree α lt} (b : α) :
-    a ∈ t → a ∈ t.insert b := by cases t; apply Rbnode.mem_insert_of_mem
-#align rbtree.mem_insert_of_mem Rbtree.mem_insert_of_mem
+#print Std.RBSet.mem_insert_of_mem /-
+theorem Std.RBSet.mem_insert_of_mem [IsStrictWeakOrder α lt] {a : α} {t : Std.RBSet α lt} (b : α) :
+    a ∈ t → a ∈ t.insert b := by cases t; apply Std.RBNode.mem_insert_of_mem
+#align rbtree.mem_insert_of_mem Std.RBSet.mem_insert_of_mem
+-/
 
-theorem equiv_or_mem_of_mem_insert {a b : α} {t : Rbtree α lt} :
-    a ∈ t.insert b → a ≈[lt]b ∨ a ∈ t := by cases t; apply Rbnode.equiv_or_mem_of_mem_insert
-#align rbtree.equiv_or_mem_of_mem_insert Rbtree.equiv_or_mem_of_mem_insert
+theorem Std.RBSet.equiv_or_mem_of_mem_insert {a b : α} {t : Std.RBSet α lt} :
+    a ∈ t.insert b → a ≈[lt]b ∨ a ∈ t := by cases t; apply Std.RBNode.equiv_or_mem_of_mem_insert
+#align rbtree.equiv_or_mem_of_mem_insert Std.RBSet.equiv_or_mem_of_mem_insert
 
-theorem incomp_or_mem_of_mem_ins {a b : α} {t : Rbtree α lt} :
+theorem Std.RBSet.incomp_or_mem_of_mem_ins {a b : α} {t : Std.RBSet α lt} :
     a ∈ t.insert b → ¬lt a b ∧ ¬lt b a ∨ a ∈ t :=
-  equiv_or_mem_of_mem_insert
-#align rbtree.incomp_or_mem_of_mem_ins Rbtree.incomp_or_mem_of_mem_ins
+  Std.RBSet.equiv_or_mem_of_mem_insert
+#align rbtree.incomp_or_mem_of_mem_ins Std.RBSet.incomp_or_mem_of_mem_ins
 
-theorem eq_or_mem_of_mem_ins [IsStrictTotalOrder α lt] {a b : α} {t : Rbtree α lt} :
+theorem Std.RBSet.eq_or_mem_of_mem_ins [IsStrictTotalOrder α lt] {a b : α} {t : Std.RBSet α lt} :
     a ∈ t.insert b → a = b ∨ a ∈ t := fun h =>
   suffices a ≈[lt]b ∨ a ∈ t by simp [eqv_lt_iff_eq] at this  <;> assumption
-  incomp_or_mem_of_mem_ins h
-#align rbtree.eq_or_mem_of_mem_ins Rbtree.eq_or_mem_of_mem_ins
+  Std.RBSet.incomp_or_mem_of_mem_ins h
+#align rbtree.eq_or_mem_of_mem_ins Std.RBSet.eq_or_mem_of_mem_ins
 
 end Dec
 
-theorem mem_of_min_eq [IsIrrefl α lt] {a : α} {t : Rbtree α lt} : t.min = some a → a ∈ t := by
-  cases t; apply Rbnode.mem_of_min_eq
-#align rbtree.mem_of_min_eq Rbtree.mem_of_min_eq
+theorem Std.RBSet.mem_of_min_eq [IsIrrefl α lt] {a : α} {t : Std.RBSet α lt} :
+    t.min = some a → a ∈ t := by cases t; apply Std.RBNode.mem_of_min_eq
+#align rbtree.mem_of_min_eq Std.RBSet.mem_of_min_eq
 
-theorem mem_of_max_eq [IsIrrefl α lt] {a : α} {t : Rbtree α lt} : t.max = some a → a ∈ t := by
-  cases t; apply Rbnode.mem_of_max_eq
-#align rbtree.mem_of_max_eq Rbtree.mem_of_max_eq
+theorem Std.RBSet.mem_of_max_eq [IsIrrefl α lt] {a : α} {t : Std.RBSet α lt} :
+    t.max = some a → a ∈ t := by cases t; apply Std.RBNode.mem_of_max_eq
+#align rbtree.mem_of_max_eq Std.RBSet.mem_of_max_eq
 
-theorem eq_leaf_of_min_eq_none {t : Rbtree α lt} : t.min = none → t = mkRbtree α lt := by cases t;
-  intro h; congr; apply Rbnode.eq_leaf_of_min_eq_none h
-#align rbtree.eq_leaf_of_min_eq_none Rbtree.eq_leaf_of_min_eq_none
+theorem Std.RBSet.eq_leaf_of_min_eq_none {t : Std.RBSet α lt} :
+    t.min = none → t = Std.mkRBSet α lt := by cases t; intro h; congr;
+  apply Std.RBNode.eq_nil_of_min_eq_none h
+#align rbtree.eq_leaf_of_min_eq_none Std.RBSet.eq_leaf_of_min_eq_none
 
-theorem eq_leaf_of_max_eq_none {t : Rbtree α lt} : t.max = none → t = mkRbtree α lt := by cases t;
-  intro h; congr; apply Rbnode.eq_leaf_of_max_eq_none h
-#align rbtree.eq_leaf_of_max_eq_none Rbtree.eq_leaf_of_max_eq_none
+theorem Std.RBSet.eq_leaf_of_max_eq_none {t : Std.RBSet α lt} :
+    t.max = none → t = Std.mkRBSet α lt := by cases t; intro h; congr;
+  apply Std.RBNode.eq_nil_of_max_eq_none h
+#align rbtree.eq_leaf_of_max_eq_none Std.RBSet.eq_leaf_of_max_eq_none
 
-theorem min_is_minimal [IsStrictWeakOrder α lt] {a : α} {t : Rbtree α lt} :
+theorem Std.RBSet.min_is_minimal [IsStrictWeakOrder α lt] {a : α} {t : Std.RBSet α lt} :
     t.min = some a → ∀ {b}, b ∈ t → a ≈[lt]b ∨ lt a b := by
   classical
   cases t
-  apply Rbnode.min_is_minimal
-  apply Rbnode.isSearchable_of_wellFormed
+  apply Std.RBNode.min_is_minimal
+  apply Std.RBNode.isSearchableOfWellFormed
   assumption
-#align rbtree.min_is_minimal Rbtree.min_is_minimal
+#align rbtree.min_is_minimal Std.RBSet.min_is_minimal
 
-theorem max_is_maximal [IsStrictWeakOrder α lt] {a : α} {t : Rbtree α lt} :
-    t.max = some a → ∀ {b}, b ∈ t → a ≈[lt]b ∨ lt b a := by cases t; apply Rbnode.max_is_maximal;
-  apply Rbnode.isSearchable_of_wellFormed; assumption
-#align rbtree.max_is_maximal Rbtree.max_is_maximal
+theorem Std.RBSet.max_is_maximal [IsStrictWeakOrder α lt] {a : α} {t : Std.RBSet α lt} :
+    t.max = some a → ∀ {b}, b ∈ t → a ≈[lt]b ∨ lt b a := by cases t;
+  apply Std.RBNode.max_is_maximal; apply Std.RBNode.isSearchableOfWellFormed; assumption
+#align rbtree.max_is_maximal Std.RBSet.max_is_maximal
 
-end Rbtree
+end Std.RBSet
 
