Mathbin/Data/Rbtree/MinMax.lean
@@ -12,66 +12,70 @@ import Mathbin.Data.Rbtree.Basic
 
 universe u
 
-namespace Rbnode
+namespace Std.RBNode
 
 variable {α : Type u} {lt : α → α → Prop}
 
-theorem mem_of_min_eq (lt : α → α → Prop) [IsIrrefl α lt] {a : α} {t : Rbnode α} :
-    t.min = some a → Mem lt a t := by
+theorem Std.RBNode.mem_of_min_eq (lt : α → α → Prop) [IsIrrefl α lt] {a : α} {t : Std.RBNode α} :
+    t.min = some a → Std.RBNode.Mem lt a t :=
+  by
   induction t
   · intros; contradiction
   all_goals
-    cases t_lchild <;> simp [Rbnode.min] <;> intro h
+    cases t_lchild <;> simp [Std.RBNode.min] <;> intro h
     · subst t_val; simp [mem, irrefl_of lt a]
     all_goals rw [mem]; simp [t_ih_lchild h]
-#align rbnode.mem_of_min_eq Rbnode.mem_of_min_eq
+#align rbnode.mem_of_min_eq Std.RBNode.mem_of_min_eq
 
-theorem mem_of_max_eq (lt : α → α → Prop) [IsIrrefl α lt] {a : α} {t : Rbnode α} :
-    t.max = some a → Mem lt a t := by
+theorem Std.RBNode.mem_of_max_eq (lt : α → α → Prop) [IsIrrefl α lt] {a : α} {t : Std.RBNode α} :
+    t.max = some a → Std.RBNode.Mem lt a t :=
+  by
   induction t
   · intros; contradiction
   all_goals
-    cases t_rchild <;> simp [Rbnode.max] <;> intro h
+    cases t_rchild <;> simp [Std.RBNode.max] <;> intro h
     · subst t_val; simp [mem, irrefl_of lt a]
     all_goals rw [mem]; simp [t_ih_rchild h]
-#align rbnode.mem_of_max_eq Rbnode.mem_of_max_eq
+#align rbnode.mem_of_max_eq Std.RBNode.mem_of_max_eq
 
 variable [IsStrictWeakOrder α lt]
 
-theorem eq_leaf_of_min_eq_none {t : Rbnode α} : t.min = none → t = leaf :=
+theorem Std.RBNode.eq_nil_of_min_eq_none {t : Std.RBNode α} : t.min = none → t = Std.RBNode.nil :=
   by
   induction t
   · intros; rfl
   all_goals
-    cases t_lchild <;> simp [Rbnode.min, false_imp_iff] <;> intro h
+    cases t_lchild <;> simp [Std.RBNode.min, false_imp_iff] <;> intro h
     all_goals have := t_ih_lchild h; contradiction
-#align rbnode.eq_leaf_of_min_eq_none Rbnode.eq_leaf_of_min_eq_none
+#align rbnode.eq_leaf_of_min_eq_none Std.RBNode.eq_nil_of_min_eq_none
 
-theorem eq_leaf_of_max_eq_none {t : Rbnode α} : t.max = none → t = leaf :=
+theorem Std.RBNode.eq_nil_of_max_eq_none {t : Std.RBNode α} : t.max = none → t = Std.RBNode.nil :=
   by
   induction t
   · intros; rfl
   all_goals
-    cases t_rchild <;> simp [Rbnode.max, false_imp_iff] <;> intro h
+    cases t_rchild <;> simp [Std.RBNode.max, false_imp_iff] <;> intro h
     all_goals have := t_ih_rchild h; contradiction
-#align rbnode.eq_leaf_of_max_eq_none Rbnode.eq_leaf_of_max_eq_none
+#align rbnode.eq_leaf_of_max_eq_none Std.RBNode.eq_nil_of_max_eq_none
 
-theorem min_is_minimal {a : α} {t : Rbnode α} :
-    ∀ {lo hi}, IsSearchable lt t lo hi → t.min = some a → ∀ {b}, Mem lt b t → a ≈[lt]b ∨ lt a b :=
+theorem Std.RBNode.min_is_minimal {a : α} {t : Std.RBNode α} :
+    ∀ {lo hi},
+      Std.RBNode.IsSearchable lt t lo hi →
+        t.min = some a → ∀ {b}, Std.RBNode.Mem lt b t → a ≈[lt]b ∨ lt a b :=
   by
   classical
   induction t
   · simp [StrictWeakOrder.Equiv]; intro _ _ hs hmin b; contradiction
   all_goals
     cases t_lchild <;> intro lo hi hs hmin b hmem
-    · simp [Rbnode.min] at hmin ; subst t_val
+    · simp [Std.RBNode.min] at hmin ; subst t_val
       simp [mem] at hmem ; cases' hmem with heqv hmem
       · left; exact heqv.swap
       · have := lt_of_mem_right hs (by constructor) hmem
         right; assumption
     all_goals
       have hs' := hs
-      cases hs; simp [Rbnode.min] at hmin 
+      cases hs; simp [Std.RBNode.min] at hmin 
       rw [mem] at hmem ; cases_type* or.1
       · exact t_ih_lchild hs_hs₁ hmin hmem
       · have hmm := mem_of_min_eq lt hmin
@@ -81,24 +85,26 @@ theorem min_is_minimal {a : α} {t : Rbnode α} :
       · have hmm := mem_of_min_eq lt hmin
         have a_lt_b := lt_of_mem_left_right hs' (by constructor) hmm hmem
         right; assumption
-#align rbnode.min_is_minimal Rbnode.min_is_minimal
+#align rbnode.min_is_minimal Std.RBNode.min_is_minimal
 
-theorem max_is_maximal {a : α} {t : Rbnode α} :
-    ∀ {lo hi}, IsSearchable lt t lo hi → t.max = some a → ∀ {b}, Mem lt b t → a ≈[lt]b ∨ lt b a :=
+theorem Std.RBNode.max_is_maximal {a : α} {t : Std.RBNode α} :
+    ∀ {lo hi},
+      Std.RBNode.IsSearchable lt t lo hi →
+        t.max = some a → ∀ {b}, Std.RBNode.Mem lt b t → a ≈[lt]b ∨ lt b a :=
   by
   classical
   induction t
   · simp [StrictWeakOrder.Equiv]; intro _ _ hs hmax b; contradiction
   all_goals
     cases t_rchild <;> intro lo hi hs hmax b hmem
-    · simp [Rbnode.max] at hmax ; subst t_val
+    · simp [Std.RBNode.max] at hmax ; subst t_val
       simp [mem] at hmem ; cases' hmem with hmem heqv
       · have := lt_of_mem_left hs (by constructor) hmem
         right; assumption
       · left; exact heqv.swap
     all_goals
       have hs' := hs
-      cases hs; simp [Rbnode.max] at hmax 
+      cases hs; simp [Std.RBNode.max] at hmax 
       rw [mem] at hmem ; cases_type* or.1
       · have hmm := mem_of_max_eq lt hmax
         have a_lt_b := lt_of_mem_left_right hs' (by constructor) hmem hmm
@@ -108,7 +114,7 @@ theorem max_is_maximal {a : α} {t : Rbnode α} :
         have a_lt_b := lt_of_incomp_of_lt hmem val_lt_a
         right; assumption
       · exact t_ih_rchild hs_hs₂ hmax hmem
-#align rbnode.max_is_maximal Rbnode.max_is_maximal
+#align rbnode.max_is_maximal Std.RBNode.max_is_maximal
 
-end Rbnode
+end Std.RBNode
 
